verified-ocaml/checker/Bytecode/InstructChecker.v
@@ -9,392 +9,1456 @@ From OCamlInterp.Manual Require Import Bytecode.Machine Bytecode.Interpret.
 From OCamlInterp.Manual Require Import Bytecode.Generated.instruct_handlers.
 From OCamlInterp.Manual Require Import Bytecode.InstructSpec.
 
-From OCamlInterp.Automatic Require Import Bytecode.InstructVerification.ACC0_correct.
-From OCamlInterp.Automatic Require Import Bytecode.InstructVerification.ACC1_correct.
-From OCamlInterp.Automatic Require Import Bytecode.InstructVerification.ACC2_correct.
-From OCamlInterp.Automatic Require Import Bytecode.InstructVerification.ACC3_correct.
-From OCamlInterp.Automatic Require Import Bytecode.InstructVerification.ACC4_correct.
-From OCamlInterp.Automatic Require Import Bytecode.InstructVerification.ACC5_correct.
-From OCamlInterp.Automatic Require Import Bytecode.InstructVerification.ACC6_correct.
-From OCamlInterp.Automatic Require Import Bytecode.InstructVerification.ACC7_correct.
-From OCamlInterp.Automatic Require Import Bytecode.InstructVerification.ACC_correct.
-From OCamlInterp.Automatic Require Import Bytecode.InstructVerification.ADDINT_correct.
-From OCamlInterp.Automatic Require Import Bytecode.InstructVerification.ANDINT_correct.
-From OCamlInterp.Automatic Require Import Bytecode.InstructVerification.APPLY1_correct.
-From OCamlInterp.Automatic Require Import Bytecode.InstructVerification.APPLY2_correct.
-From OCamlInterp.Automatic Require Import Bytecode.InstructVerification.APPLY3_correct.
-From OCamlInterp.Automatic Require Import Bytecode.InstructVerification.APPLY_correct.
-From OCamlInterp.Automatic Require Import Bytecode.InstructVerification.APPTERM1_correct.
-From OCamlInterp.Automatic Require Import Bytecode.InstructVerification.APPTERM2_correct.
-From OCamlInterp.Automatic Require Import Bytecode.InstructVerification.APPTERM3_correct.
-From OCamlInterp.Automatic Require Import Bytecode.InstructVerification.APPTERM_correct.
-From OCamlInterp.Automatic Require Import Bytecode.InstructVerification.ASRINT_correct.
-From OCamlInterp.Automatic Require Import Bytecode.InstructVerification.ASSIGN_correct.
-From OCamlInterp.Automatic Require Import Bytecode.InstructVerification.ATOM0_correct.
-From OCamlInterp.Automatic Require Import Bytecode.InstructVerification.ATOM_correct.
-From OCamlInterp.Automatic Require Import Bytecode.InstructVerification.BEQ_correct.
-From OCamlInterp.Automatic Require Import Bytecode.InstructVerification.BGEINT_correct.
-From OCamlInterp.Automatic Require Import Bytecode.InstructVerification.BGTINT_correct.
-From OCamlInterp.Automatic Require Import Bytecode.InstructVerification.BLEINT_correct.
-From OCamlInterp.Automatic Require Import Bytecode.InstructVerification.BLTINT_correct.
-From OCamlInterp.Automatic Require Import Bytecode.InstructVerification.BNEQ_correct.
-From OCamlInterp.Automatic Require Import Bytecode.InstructVerification.BOOLNOT_correct.
-From OCamlInterp.Automatic Require Import Bytecode.InstructVerification.BRANCHIFNOT_correct.
-From OCamlInterp.Automatic Require Import Bytecode.InstructVerification.BRANCHIF_correct.
-From OCamlInterp.Automatic Require Import Bytecode.InstructVerification.BRANCH_correct.
-From OCamlInterp.Automatic Require Import Bytecode.InstructVerification.BREAK_correct.
-From OCamlInterp.Automatic Require Import Bytecode.InstructVerification.BUGEINT_correct.
-From OCamlInterp.Automatic Require Import Bytecode.InstructVerification.BULTINT_correct.
-From OCamlInterp.Automatic Require Import Bytecode.InstructVerification.CHECK_SIGNALS_correct.
-From OCamlInterp.Automatic Require Import Bytecode.InstructVerification.CLOSUREREC_correct.
-From OCamlInterp.Automatic Require Import Bytecode.InstructVerification.CLOSURE_correct.
-From OCamlInterp.Automatic Require Import Bytecode.InstructVerification.CONST0_correct.
-From OCamlInterp.Automatic Require Import Bytecode.InstructVerification.CONST1_correct.
-From OCamlInterp.Automatic Require Import Bytecode.InstructVerification.CONST2_correct.
-From OCamlInterp.Automatic Require Import Bytecode.InstructVerification.CONST3_correct.
-From OCamlInterp.Automatic Require Import Bytecode.InstructVerification.CONSTINT_correct.
-From OCamlInterp.Automatic Require Import Bytecode.InstructVerification.C_CALL1_correct.
-From OCamlInterp.Automatic Require Import Bytecode.InstructVerification.C_CALL2_correct.
-From OCamlInterp.Automatic Require Import Bytecode.InstructVerification.C_CALL3_correct.
-From OCamlInterp.Automatic Require Import Bytecode.InstructVerification.C_CALL4_correct.
-From OCamlInterp.Automatic Require Import Bytecode.InstructVerification.C_CALL5_correct.
-From OCamlInterp.Automatic Require Import Bytecode.InstructVerification.C_CALLN_correct.
-From OCamlInterp.Automatic Require Import Bytecode.InstructVerification.DIVINT_correct.
-From OCamlInterp.Automatic Require Import Bytecode.InstructVerification.ENVACC1_correct.
-From OCamlInterp.Automatic Require Import Bytecode.InstructVerification.ENVACC2_correct.
-From OCamlInterp.Automatic Require Import Bytecode.InstructVerification.ENVACC3_correct.
-From OCamlInterp.Automatic Require Import Bytecode.InstructVerification.ENVACC4_correct.
-From OCamlInterp.Automatic Require Import Bytecode.InstructVerification.ENVACC_correct.
-From OCamlInterp.Automatic Require Import Bytecode.InstructVerification.EQ_correct.
-From OCamlInterp.Automatic Require Import Bytecode.InstructVerification.EVENT_correct.
-From OCamlInterp.Automatic Require Import Bytecode.InstructVerification.GEINT_correct.
-From OCamlInterp.Automatic Require Import Bytecode.InstructVerification.GETBYTESCHAR_correct.
-From OCamlInterp.Automatic Require Import Bytecode.InstructVerification.GETDYNMET_correct.
-From OCamlInterp.Automatic Require Import Bytecode.InstructVerification.GETFIELD0_correct.
-From OCamlInterp.Automatic Require Import Bytecode.InstructVerification.GETFIELD1_correct.
-From OCamlInterp.Automatic Require Import Bytecode.InstructVerification.GETFIELD2_correct.
-From OCamlInterp.Automatic Require Import Bytecode.InstructVerification.GETFIELD3_correct.
-From OCamlInterp.Automatic Require Import Bytecode.InstructVerification.GETFIELD_correct.
-From OCamlInterp.Automatic Require Import Bytecode.InstructVerification.GETFLOATFIELD_correct.
-From OCamlInterp.Automatic Require Import Bytecode.InstructVerification.GETGLOBALFIELD_correct.
-From OCamlInterp.Automatic Require Import Bytecode.InstructVerification.GETGLOBAL_correct.
-From OCamlInterp.Automatic Require Import Bytecode.InstructVerification.GETMETHOD_correct.
-From OCamlInterp.Automatic Require Import Bytecode.InstructVerification.GETPUBMET_correct.
-From OCamlInterp.Automatic Require Import Bytecode.InstructVerification.GETSTRINGCHAR_correct.
-From OCamlInterp.Automatic Require Import Bytecode.InstructVerification.GETVECTITEM_correct.
-From OCamlInterp.Automatic Require Import Bytecode.InstructVerification.GRAB_correct.
-From OCamlInterp.Automatic Require Import Bytecode.InstructVerification.GTINT_correct.
-From OCamlInterp.Automatic Require Import Bytecode.InstructVerification.ISINT_correct.
-From OCamlInterp.Automatic Require Import Bytecode.InstructVerification.LEINT_correct.
-From OCamlInterp.Automatic Require Import Bytecode.InstructVerification.LSLINT_correct.
-From OCamlInterp.Automatic Require Import Bytecode.InstructVerification.LSRINT_correct.
-From OCamlInterp.Automatic Require Import Bytecode.InstructVerification.LTINT_correct.
-From OCamlInterp.Automatic Require Import Bytecode.InstructVerification.MAKEBLOCK1_correct.
-From OCamlInterp.Automatic Require Import Bytecode.InstructVerification.MAKEBLOCK2_correct.
-From OCamlInterp.Automatic Require Import Bytecode.InstructVerification.MAKEBLOCK3_correct.
-From OCamlInterp.Automatic Require Import Bytecode.InstructVerification.MAKEBLOCK_correct.
-From OCamlInterp.Automatic Require Import Bytecode.InstructVerification.MAKEFLOATBLOCK_correct.
-From OCamlInterp.Automatic Require Import Bytecode.InstructVerification.MODINT_correct.
-From OCamlInterp.Automatic Require Import Bytecode.InstructVerification.MULINT_correct.
-From OCamlInterp.Automatic Require Import Bytecode.InstructVerification.NEGINT_correct.
-From OCamlInterp.Automatic Require Import Bytecode.InstructVerification.NEQ_correct.
-From OCamlInterp.Automatic Require Import Bytecode.InstructVerification.OFFSETCLOSURE0_correct.
-From OCamlInterp.Automatic Require Import Bytecode.InstructVerification.OFFSETCLOSURE2_correct.
-From OCamlInterp.Automatic Require Import Bytecode.InstructVerification.OFFSETCLOSUREM2_correct.
-From OCamlInterp.Automatic Require Import Bytecode.InstructVerification.OFFSETCLOSURE_correct.
-From OCamlInterp.Automatic Require Import Bytecode.InstructVerification.OFFSETINT_correct.
-From OCamlInterp.Automatic Require Import Bytecode.InstructVerification.OFFSETREF_correct.
-From OCamlInterp.Automatic Require Import Bytecode.InstructVerification.ORINT_correct.
-From OCamlInterp.Automatic Require Import Bytecode.InstructVerification.PERFORM_correct.
-From OCamlInterp.Automatic Require Import Bytecode.InstructVerification.POPTRAP_correct.
-From OCamlInterp.Automatic Require Import Bytecode.InstructVerification.POP_correct.
-From OCamlInterp.Automatic Require Import Bytecode.InstructVerification.PUSHACC1_correct.
-From OCamlInterp.Automatic Require Import Bytecode.InstructVerification.PUSHACC2_correct.
-From OCamlInterp.Automatic Require Import Bytecode.InstructVerification.PUSHACC3_correct.
-From OCamlInterp.Automatic Require Import Bytecode.InstructVerification.PUSHACC4_correct.
-From OCamlInterp.Automatic Require Import Bytecode.InstructVerification.PUSHACC5_correct.
-From OCamlInterp.Automatic Require Import Bytecode.InstructVerification.PUSHACC6_correct.
-From OCamlInterp.Automatic Require Import Bytecode.InstructVerification.PUSHACC7_correct.
-From OCamlInterp.Automatic Require Import Bytecode.InstructVerification.PUSHATOM0_correct.
-From OCamlInterp.Automatic Require Import Bytecode.InstructVerification.PUSHATOM_correct.
-From OCamlInterp.Automatic Require Import Bytecode.InstructVerification.PUSHCONST0_correct.
-From OCamlInterp.Automatic Require Import Bytecode.InstructVerification.PUSHCONST1_correct.
-From OCamlInterp.Automatic Require Import Bytecode.InstructVerification.PUSHCONST2_correct.
-From OCamlInterp.Automatic Require Import Bytecode.InstructVerification.PUSHCONST3_correct.
-From OCamlInterp.Automatic Require Import Bytecode.InstructVerification.PUSHCONSTINT_correct.
-From OCamlInterp.Automatic Require Import Bytecode.InstructVerification.PUSHENVACC1_correct.
-From OCamlInterp.Automatic Require Import Bytecode.InstructVerification.PUSHENVACC2_correct.
-From OCamlInterp.Automatic Require Import Bytecode.InstructVerification.PUSHENVACC3_correct.
-From OCamlInterp.Automatic Require Import Bytecode.InstructVerification.PUSHENVACC4_correct.
-From OCamlInterp.Automatic Require Import Bytecode.InstructVerification.PUSHENVACC_correct.
-From OCamlInterp.Automatic Require Import Bytecode.InstructVerification.PUSHGETGLOBALFIELD_correct.
-From OCamlInterp.Automatic Require Import Bytecode.InstructVerification.PUSHGETGLOBAL_correct.
-From OCamlInterp.Automatic Require Import Bytecode.InstructVerification.PUSHOFFSETCLOSURE0_correct.
-From OCamlInterp.Automatic Require Import Bytecode.InstructVerification.PUSHOFFSETCLOSURE2_correct.
-From OCamlInterp.Automatic Require Import Bytecode.InstructVerification.PUSHOFFSETCLOSUREM2_correct.
-From OCamlInterp.Automatic Require Import Bytecode.InstructVerification.PUSHOFFSETCLOSURE_correct.
-From OCamlInterp.Automatic Require Import Bytecode.InstructVerification.PUSHTRAP_correct.
-From OCamlInterp.Automatic Require Import Bytecode.InstructVerification.PUSH_RETADDR_correct.
-From OCamlInterp.Automatic Require Import Bytecode.InstructVerification.PUSH_correct.
-From OCamlInterp.Automatic Require Import Bytecode.InstructVerification.RAISE_NOTRACE_correct.
-From OCamlInterp.Automatic Require Import Bytecode.InstructVerification.RAISE_correct.
-From OCamlInterp.Automatic Require Import Bytecode.InstructVerification.REPERFORMTERM_correct.
-From OCamlInterp.Automatic Require Import Bytecode.InstructVerification.RERAISE_correct.
-From OCamlInterp.Automatic Require Import Bytecode.InstructVerification.RESTART_correct.
-From OCamlInterp.Automatic Require Import Bytecode.InstructVerification.RESUMETERM_correct.
-From OCamlInterp.Automatic Require Import Bytecode.InstructVerification.RESUME_correct.
-From OCamlInterp.Automatic Require Import Bytecode.InstructVerification.RETURN_correct.
-From OCamlInterp.Automatic Require Import Bytecode.InstructVerification.SETBYTESCHAR_correct.
-From OCamlInterp.Automatic Require Import Bytecode.InstructVerification.SETFIELD0_correct.
-From OCamlInterp.Automatic Require Import Bytecode.InstructVerification.SETFIELD1_correct.
-From OCamlInterp.Automatic Require Import Bytecode.InstructVerification.SETFIELD2_correct.
-From OCamlInterp.Automatic Require Import Bytecode.InstructVerification.SETFIELD3_correct.
-From OCamlInterp.Automatic Require Import Bytecode.InstructVerification.SETFIELD_correct.
-From OCamlInterp.Automatic Require Import Bytecode.InstructVerification.SETFLOATFIELD_correct.
-From OCamlInterp.Automatic Require Import Bytecode.InstructVerification.SETGLOBAL_correct.
-From OCamlInterp.Automatic Require Import Bytecode.InstructVerification.SETVECTITEM_correct.
-From OCamlInterp.Automatic Require Import Bytecode.InstructVerification.STOP_correct.
-From OCamlInterp.Automatic Require Import Bytecode.InstructVerification.SUBINT_correct.
-From OCamlInterp.Automatic Require Import Bytecode.InstructVerification.SWITCH_correct.
-From OCamlInterp.Automatic Require Import Bytecode.InstructVerification.UGEINT_correct.
-From OCamlInterp.Automatic Require Import Bytecode.InstructVerification.ULTINT_correct.
-From OCamlInterp.Automatic Require Import Bytecode.InstructVerification.VECTLENGTH_correct.
-From OCamlInterp.Automatic Require Import Bytecode.InstructVerification.XORINT_correct.
+From OCamlInterp.Automatic Require Bytecode.InstructVerification.ACC0_correct.
+From OCamlInterp.Automatic Require Bytecode.InstructVerification.ACC1_correct.
+From OCamlInterp.Automatic Require Bytecode.InstructVerification.ACC2_correct.
+From OCamlInterp.Automatic Require Bytecode.InstructVerification.ACC3_correct.
+From OCamlInterp.Automatic Require Bytecode.InstructVerification.ACC4_correct.
+From OCamlInterp.Automatic Require Bytecode.InstructVerification.ACC5_correct.
+From OCamlInterp.Automatic Require Bytecode.InstructVerification.ACC6_correct.
+From OCamlInterp.Automatic Require Bytecode.InstructVerification.ACC7_correct.
+From OCamlInterp.Automatic Require Bytecode.InstructVerification.ACC_correct.
+From OCamlInterp.Automatic Require Bytecode.InstructVerification.ADDINT_correct.
+From OCamlInterp.Automatic Require Bytecode.InstructVerification.ANDINT_correct.
+From OCamlInterp.Automatic Require Bytecode.InstructVerification.APPLY1_correct.
+From OCamlInterp.Automatic Require Bytecode.InstructVerification.APPLY2_correct.
+From OCamlInterp.Automatic Require Bytecode.InstructVerification.APPLY3_correct.
+From OCamlInterp.Automatic Require Bytecode.InstructVerification.APPLY_correct.
+From OCamlInterp.Automatic Require Bytecode.InstructVerification.APPTERM1_correct.
+From OCamlInterp.Automatic Require Bytecode.InstructVerification.APPTERM2_correct.
+From OCamlInterp.Automatic Require Bytecode.InstructVerification.APPTERM3_correct.
+From OCamlInterp.Automatic Require Bytecode.InstructVerification.APPTERM_correct.
+From OCamlInterp.Automatic Require Bytecode.InstructVerification.ASRINT_correct.
+From OCamlInterp.Automatic Require Bytecode.InstructVerification.ASSIGN_correct.
+From OCamlInterp.Automatic Require Bytecode.InstructVerification.ATOM0_correct.
+From OCamlInterp.Automatic Require Bytecode.InstructVerification.ATOM_correct.
+From OCamlInterp.Automatic Require Bytecode.InstructVerification.BEQ_correct.
+From OCamlInterp.Automatic Require Bytecode.InstructVerification.BGEINT_correct.
+From OCamlInterp.Automatic Require Bytecode.InstructVerification.BGTINT_correct.
+From OCamlInterp.Automatic Require Bytecode.InstructVerification.BLEINT_correct.
+From OCamlInterp.Automatic Require Bytecode.InstructVerification.BLTINT_correct.
+From OCamlInterp.Automatic Require Bytecode.InstructVerification.BNEQ_correct.
+From OCamlInterp.Automatic Require Bytecode.InstructVerification.BOOLNOT_correct.
+From OCamlInterp.Automatic Require Bytecode.InstructVerification.BRANCHIFNOT_correct.
+From OCamlInterp.Automatic Require Bytecode.InstructVerification.BRANCHIF_correct.
+From OCamlInterp.Automatic Require Bytecode.InstructVerification.BRANCH_correct.
+From OCamlInterp.Automatic Require Bytecode.InstructVerification.BREAK_correct.
+From OCamlInterp.Automatic Require Bytecode.InstructVerification.BUGEINT_correct.
+From OCamlInterp.Automatic Require Bytecode.InstructVerification.BULTINT_correct.
+From OCamlInterp.Automatic Require Bytecode.InstructVerification.CHECK_SIGNALS_correct.
+From OCamlInterp.Automatic Require Bytecode.InstructVerification.CLOSUREREC_correct.
+From OCamlInterp.Automatic Require Bytecode.InstructVerification.CLOSURE_correct.
+From OCamlInterp.Automatic Require Bytecode.InstructVerification.CONST0_correct.
+From OCamlInterp.Automatic Require Bytecode.InstructVerification.CONST1_correct.
+From OCamlInterp.Automatic Require Bytecode.InstructVerification.CONST2_correct.
+From OCamlInterp.Automatic Require Bytecode.InstructVerification.CONST3_correct.
+From OCamlInterp.Automatic Require Bytecode.InstructVerification.CONSTINT_correct.
+From OCamlInterp.Automatic Require Bytecode.InstructVerification.C_CALL1_correct.
+From OCamlInterp.Automatic Require Bytecode.InstructVerification.C_CALL2_correct.
+From OCamlInterp.Automatic Require Bytecode.InstructVerification.C_CALL3_correct.
+From OCamlInterp.Automatic Require Bytecode.InstructVerification.C_CALL4_correct.
+From OCamlInterp.Automatic Require Bytecode.InstructVerification.C_CALL5_correct.
+From OCamlInterp.Automatic Require Bytecode.InstructVerification.C_CALLN_correct.
+From OCamlInterp.Automatic Require Bytecode.InstructVerification.DIVINT_correct.
+From OCamlInterp.Automatic Require Bytecode.InstructVerification.ENVACC1_correct.
+From OCamlInterp.Automatic Require Bytecode.InstructVerification.ENVACC2_correct.
+From OCamlInterp.Automatic Require Bytecode.InstructVerification.ENVACC3_correct.
+From OCamlInterp.Automatic Require Bytecode.InstructVerification.ENVACC4_correct.
+From OCamlInterp.Automatic Require Bytecode.InstructVerification.ENVACC_correct.
+From OCamlInterp.Automatic Require Bytecode.InstructVerification.EQ_correct.
+From OCamlInterp.Automatic Require Bytecode.InstructVerification.EVENT_correct.
+From OCamlInterp.Automatic Require Bytecode.InstructVerification.GEINT_correct.
+From OCamlInterp.Automatic Require Bytecode.InstructVerification.GETBYTESCHAR_correct.
+From OCamlInterp.Automatic Require Bytecode.InstructVerification.GETDYNMET_correct.
+From OCamlInterp.Automatic Require Bytecode.InstructVerification.GETFIELD0_correct.
+From OCamlInterp.Automatic Require Bytecode.InstructVerification.GETFIELD1_correct.
+From OCamlInterp.Automatic Require Bytecode.InstructVerification.GETFIELD2_correct.
+From OCamlInterp.Automatic Require Bytecode.InstructVerification.GETFIELD3_correct.
+From OCamlInterp.Automatic Require Bytecode.InstructVerification.GETFIELD_correct.
+From OCamlInterp.Automatic Require Bytecode.InstructVerification.GETFLOATFIELD_correct.
+From OCamlInterp.Automatic Require Bytecode.InstructVerification.GETGLOBALFIELD_correct.
+From OCamlInterp.Automatic Require Bytecode.InstructVerification.GETGLOBAL_correct.
+From OCamlInterp.Automatic Require Bytecode.InstructVerification.GETMETHOD_correct.
+From OCamlInterp.Automatic Require Bytecode.InstructVerification.GETPUBMET_correct.
+From OCamlInterp.Automatic Require Bytecode.InstructVerification.GETSTRINGCHAR_correct.
+From OCamlInterp.Automatic Require Bytecode.InstructVerification.GETVECTITEM_correct.
+From OCamlInterp.Automatic Require Bytecode.InstructVerification.GRAB_correct.
+From OCamlInterp.Automatic Require Bytecode.InstructVerification.GTINT_correct.
+From OCamlInterp.Automatic Require Bytecode.InstructVerification.ISINT_correct.
+From OCamlInterp.Automatic Require Bytecode.InstructVerification.LEINT_correct.
+From OCamlInterp.Automatic Require Bytecode.InstructVerification.LSLINT_correct.
+From OCamlInterp.Automatic Require Bytecode.InstructVerification.LSRINT_correct.
+From OCamlInterp.Automatic Require Bytecode.InstructVerification.LTINT_correct.
+From OCamlInterp.Automatic Require Bytecode.InstructVerification.MAKEBLOCK1_correct.
+From OCamlInterp.Automatic Require Bytecode.InstructVerification.MAKEBLOCK2_correct.
+From OCamlInterp.Automatic Require Bytecode.InstructVerification.MAKEBLOCK3_correct.
+From OCamlInterp.Automatic Require Bytecode.InstructVerification.MAKEBLOCK_correct.
+From OCamlInterp.Automatic Require Bytecode.InstructVerification.MAKEFLOATBLOCK_correct.
+From OCamlInterp.Automatic Require Bytecode.InstructVerification.MODINT_correct.
+From OCamlInterp.Automatic Require Bytecode.InstructVerification.MULINT_correct.
+From OCamlInterp.Automatic Require Bytecode.InstructVerification.NEGINT_correct.
+From OCamlInterp.Automatic Require Bytecode.InstructVerification.NEQ_correct.
+From OCamlInterp.Automatic Require Bytecode.InstructVerification.OFFSETCLOSURE0_correct.
+From OCamlInterp.Automatic Require Bytecode.InstructVerification.OFFSETCLOSURE2_correct.
+From OCamlInterp.Automatic Require Bytecode.InstructVerification.OFFSETCLOSUREM2_correct.
+From OCamlInterp.Automatic Require Bytecode.InstructVerification.OFFSETCLOSURE_correct.
+From OCamlInterp.Automatic Require Bytecode.InstructVerification.OFFSETINT_correct.
+From OCamlInterp.Automatic Require Bytecode.InstructVerification.OFFSETREF_correct.
+From OCamlInterp.Automatic Require Bytecode.InstructVerification.ORINT_correct.
+From OCamlInterp.Automatic Require Bytecode.InstructVerification.PERFORM_correct.
+From OCamlInterp.Automatic Require Bytecode.InstructVerification.POPTRAP_correct.
+From OCamlInterp.Automatic Require Bytecode.InstructVerification.POP_correct.
+From OCamlInterp.Automatic Require Bytecode.InstructVerification.PUSHACC1_correct.
+From OCamlInterp.Automatic Require Bytecode.InstructVerification.PUSHACC2_correct.
+From OCamlInterp.Automatic Require Bytecode.InstructVerification.PUSHACC3_correct.
+From OCamlInterp.Automatic Require Bytecode.InstructVerification.PUSHACC4_correct.
+From OCamlInterp.Automatic Require Bytecode.InstructVerification.PUSHACC5_correct.
+From OCamlInterp.Automatic Require Bytecode.InstructVerification.PUSHACC6_correct.
+From OCamlInterp.Automatic Require Bytecode.InstructVerification.PUSHACC7_correct.
+From OCamlInterp.Automatic Require Bytecode.InstructVerification.PUSHATOM0_correct.
+From OCamlInterp.Automatic Require Bytecode.InstructVerification.PUSHATOM_correct.
+From OCamlInterp.Automatic Require Bytecode.InstructVerification.PUSHCONST0_correct.
+From OCamlInterp.Automatic Require Bytecode.InstructVerification.PUSHCONST1_correct.
+From OCamlInterp.Automatic Require Bytecode.InstructVerification.PUSHCONST2_correct.
+From OCamlInterp.Automatic Require Bytecode.InstructVerification.PUSHCONST3_correct.
+From OCamlInterp.Automatic Require Bytecode.InstructVerification.PUSHCONSTINT_correct.
+From OCamlInterp.Automatic Require Bytecode.InstructVerification.PUSHENVACC1_correct.
+From OCamlInterp.Automatic Require Bytecode.InstructVerification.PUSHENVACC2_correct.
+From OCamlInterp.Automatic Require Bytecode.InstructVerification.PUSHENVACC3_correct.
+From OCamlInterp.Automatic Require Bytecode.InstructVerification.PUSHENVACC4_correct.
+From OCamlInterp.Automatic Require Bytecode.InstructVerification.PUSHENVACC_correct.
+From OCamlInterp.Automatic Require Bytecode.InstructVerification.PUSHGETGLOBALFIELD_correct.
+From OCamlInterp.Automatic Require Bytecode.InstructVerification.PUSHGETGLOBAL_correct.
+From OCamlInterp.Automatic Require Bytecode.InstructVerification.PUSHOFFSETCLOSURE0_correct.
+From OCamlInterp.Automatic Require Bytecode.InstructVerification.PUSHOFFSETCLOSURE2_correct.
+From OCamlInterp.Automatic Require Bytecode.InstructVerification.PUSHOFFSETCLOSUREM2_correct.
+From OCamlInterp.Automatic Require Bytecode.InstructVerification.PUSHOFFSETCLOSURE_correct.
+From OCamlInterp.Automatic Require Bytecode.InstructVerification.PUSHTRAP_correct.
+From OCamlInterp.Automatic Require Bytecode.InstructVerification.PUSH_RETADDR_correct.
+From OCamlInterp.Automatic Require Bytecode.InstructVerification.PUSH_correct.
+From OCamlInterp.Automatic Require Bytecode.InstructVerification.RAISE_NOTRACE_correct.
+From OCamlInterp.Automatic Require Bytecode.InstructVerification.RAISE_correct.
+From OCamlInterp.Automatic Require Bytecode.InstructVerification.REPERFORMTERM_correct.
+From OCamlInterp.Automatic Require Bytecode.InstructVerification.RERAISE_correct.
+From OCamlInterp.Automatic Require Bytecode.InstructVerification.RESTART_correct.
+From OCamlInterp.Automatic Require Bytecode.InstructVerification.RESUMETERM_correct.
+From OCamlInterp.Automatic Require Bytecode.InstructVerification.RESUME_correct.
+From OCamlInterp.Automatic Require Bytecode.InstructVerification.RETURN_correct.
+From OCamlInterp.Automatic Require Bytecode.InstructVerification.SETBYTESCHAR_correct.
+From OCamlInterp.Automatic Require Bytecode.InstructVerification.SETFIELD0_correct.
+From OCamlInterp.Automatic Require Bytecode.InstructVerification.SETFIELD1_correct.
+From OCamlInterp.Automatic Require Bytecode.InstructVerification.SETFIELD2_correct.
+From OCamlInterp.Automatic Require Bytecode.InstructVerification.SETFIELD3_correct.
+From OCamlInterp.Automatic Require Bytecode.InstructVerification.SETFIELD_correct.
+From OCamlInterp.Automatic Require Bytecode.InstructVerification.SETFLOATFIELD_correct.
+From OCamlInterp.Automatic Require Bytecode.InstructVerification.SETGLOBAL_correct.
+From OCamlInterp.Automatic Require Bytecode.InstructVerification.SETVECTITEM_correct.
+From OCamlInterp.Automatic Require Bytecode.InstructVerification.STOP_correct.
+From OCamlInterp.Automatic Require Bytecode.InstructVerification.SUBINT_correct.
+From OCamlInterp.Automatic Require Bytecode.InstructVerification.SWITCH_correct.
+From OCamlInterp.Automatic Require Bytecode.InstructVerification.UGEINT_correct.
+From OCamlInterp.Automatic Require Bytecode.InstructVerification.ULTINT_correct.
+From OCamlInterp.Automatic Require Bytecode.InstructVerification.VECTLENGTH_correct.
+From OCamlInterp.Automatic Require Bytecode.InstructVerification.XORINT_correct.
 
 
 Module InstructVerification <: InstructVerificationSpec.
 
-  Definition correct_ACC0 := verify_ACC0_compl_comp.
-  Definition correct_ACC1 := verify_ACC1.
-  Definition correct_ACC2 := verify_ACC2.
-  Definition correct_ACC3 := verify_ACC3.
-  Definition correct_ACC4 := verify_ACC4.
-  Definition correct_ACC5 := verify_ACC5.
-  Definition correct_ACC6 := verify_ACC6.
-  Definition correct_ACC7 := verify_ACC7.
+  Definition correct_ACC0 := ACC0_correct.verify_ACC0_compl_comp.
+  Definition correct_ACC1 := ACC1_correct.verify_ACC1.
+  Definition correct_ACC2 := ACC2_correct.verify_ACC2.
+  Definition correct_ACC3 := ACC3_correct.verify_ACC3.
+  Definition correct_ACC4 := ACC4_correct.verify_ACC4.
+  Definition correct_ACC5 := ACC5_correct.verify_ACC5.
+  Definition correct_ACC6 := ACC6_correct.verify_ACC6.
+  Definition correct_ACC7 := ACC7_correct.verify_ACC7.
   Definition correct_ACC :
     forall n,
     Z.of_nat n < Int.half_modulus ->
     handler_correct (handle_ACC n) f_instr_ACC
       (code_at (Int.repr (Z.of_nat n)))
       (fun _ s => nth_error s.(Machine.stack) n = None) (fun _ => False) (fun _ _ _ => False)
-    := verify_ACC_handler_correct.
-  Definition correct_ADDINT := verify_ADDINT_compl_comp.
-  Definition correct_ANDINT := verify_ANDINT_correct.
-  Definition correct_APPLY1 := verify_APPLY1_correct.
-  Definition correct_APPLY2 := verify_APPLY2_correct.
-  Definition correct_APPLY3 := verify_APPLY3_correct.
-  Definition correct_APPLY := verify_APPLY_correct.
-  Definition correct_APPTERM1 := verify_APPTERM1_correct.
-  Definition correct_APPTERM2 := verify_APPTERM2_correct.
-  Definition correct_APPTERM3 := verify_APPTERM3_correct.
-  Definition correct_APPTERM := verify_APPTERM_correct.
-  Definition correct_ASRINT := verify_ASRINT_handler_correct.
-  Definition correct_ASSIGN := verify_ASSIGN_correct.
-  Definition correct_ATOM0 := verify_ATOM0_correct.
-  Definition correct_ATOM := verify_ATOM_correct.
+    := ACC_correct.verify_ACC_handler_correct.
+  Definition correct_ADDINT := ADDINT_correct.verify_ADDINT_compl_comp.
+  Definition correct_ANDINT := ANDINT_correct.verify_ANDINT_correct.
+  Definition correct_APPLY1 := APPLY1_correct.verify_APPLY1_correct.
+  Definition correct_APPLY2 := APPLY2_correct.verify_APPLY2_correct.
+  Definition correct_APPLY3 := APPLY3_correct.verify_APPLY3_correct.
+  Definition correct_APPLY := APPLY_correct.verify_APPLY_correct.
+  Definition correct_APPTERM1 := APPTERM1_correct.verify_APPTERM1_correct.
+  Definition correct_APPTERM2 := APPTERM2_correct.verify_APPTERM2_correct.
+  Definition correct_APPTERM3 := APPTERM3_correct.verify_APPTERM3_correct.
+  Definition correct_APPTERM := APPTERM_correct.verify_APPTERM_correct.
+  Definition correct_ASRINT := ASRINT_correct.verify_ASRINT_handler_correct.
+  Definition correct_ASSIGN := ASSIGN_correct.verify_ASSIGN_correct.
+  Definition correct_ATOM0 := ATOM0_correct.verify_ATOM0_correct.
+  Definition correct_ATOM := ATOM_correct.verify_ATOM_correct.
   Definition correct_BEQ :
     forall n target,
     Int.min_signed <= n <= Int.max_signed ->
     handler_correct (handle_BEQ n target) f_instr_BEQ
       (pre_and (pre_and (pre_and code_ne_struct (code_at (Int.repr n))) (branch_offset_at target)) (pre_and accu_signed_int accu_is_long))
       (fun _ _ => False) (fun _ => False) (fun _ _ _ => False)
-    := verify_BEQ_handler_correct.
+    := BEQ_correct.verify_BEQ_handler_correct.
   Definition correct_BGEINT :
     forall n target,
     Int.min_signed <= n <= Int.max_signed ->
     handler_correct (handle_BGEINT n target) f_instr_BGEINT
       (pre_and (pre_and (pre_and code_ne_struct (code_at (Int.repr n))) (branch_offset_at target)) (pre_and accu_signed_int accu_is_long))
       (fun msg s => msg = "BGEINT: not an integer"%string /\ match Machine.accu s with Val_int _ => False | _ => True end) (fun _ => False) (fun _ _ _ => False)
-    := verify_BGEINT_handler_correct.
+    := BGEINT_correct.verify_BGEINT_handler_correct.
   Definition correct_BGTINT :
     forall n target,
     Int.min_signed <= n <= Int.max_signed ->
     handler_correct (handle_BGTINT n target) f_instr_BGTINT
       (pre_and (pre_and (pre_and code_ne_struct (code_at (Int.repr n))) (branch_offset_at target)) (pre_and accu_signed_int accu_is_long))
       (fun msg s => msg = "BGTINT: not an integer"%string /\ match Machine.accu s with Val_int _ => False | _ => True end) (fun _ => False) (fun _ _ _ => False)
-    := verify_BGTINT_handler_correct.
+    := BGTINT_correct.verify_BGTINT_handler_correct.
   Definition correct_BLEINT :
     forall n target,
     Int.min_signed <= n <= Int.max_signed ->
     handler_correct (handle_BLEINT n target) f_instr_BLEINT
       (pre_and (pre_and (pre_and code_ne_struct (code_at (Int.repr n))) (branch_offset_at target)) (pre_and accu_signed_int accu_is_long))
       (fun msg s => msg = "BLEINT: not an integer"%string /\ match Machine.accu s with Val_int _ => False | _ => True end) (fun _ => False) (fun _ _ _ => False)
-    := verify_BLEINT_handler_correct.
+    := BLEINT_correct.verify_BLEINT_handler_correct.
   Definition correct_BLTINT :
     forall n target,
     Int.min_signed <= n <= Int.max_signed ->
     handler_correct (handle_BLTINT n target) f_instr_BLTINT
       (pre_and (pre_and (pre_and code_ne_struct (code_at (Int.repr n))) (branch_offset_at target)) (pre_and accu_signed_int accu_is_long))
       (fun msg s => msg = "BLTINT: not an integer"%string /\ match Machine.accu s with Val_int _ => False | _ => True end) (fun _ => False) (fun _ _ _ => False)
-    := verify_BLTINT_handler_correct.
+    := BLTINT_correct.verify_BLTINT_handler_correct.
   Definition correct_BNEQ :
     forall n target,
     Int.min_signed <= n <= Int.max_signed ->
     handler_correct (handle_BNEQ n target) f_instr_BNEQ
       (pre_and (pre_and (pre_and code_ne_struct (code_at (Int.repr n))) (branch_offset_at target)) (pre_and accu_signed_int accu_is_long))
       (fun _ _ => False) (fun _ => False) (fun _ _ _ => False)
-    := verify_BNEQ_handler_correct.
-  Definition correct_BOOLNOT := verify_BOOLNOT_handler_correct.
-  Definition correct_BRANCHIFNOT := verify_BRANCHIFNOT_correct.
-  Definition correct_BRANCHIF := verify_BRANCHIF_correct.
+    := BNEQ_correct.verify_BNEQ_handler_correct.
+  Definition correct_BOOLNOT := BOOLNOT_correct.verify_BOOLNOT_handler_correct.
+  Definition correct_BRANCHIFNOT := BRANCHIFNOT_correct.verify_BRANCHIFNOT_correct.
+  Definition correct_BRANCHIF := BRANCHIF_correct.verify_BRANCHIF_correct.
   Definition correct_BRANCH :
     forall target,
     handler_correct (fun _ s => handle_BRANCH target s) f_instr_BRANCH
       code_loadable
       (fun _ _ => False) (fun _ => False) (fun _ _ _ => False)
-    := verify_BRANCH_handler_correct.
-  Definition correct_BREAK := verify_BREAK_correct.
+    := BRANCH_correct.verify_BRANCH_handler_correct.
+  Definition correct_BREAK := BREAK_correct.verify_BREAK_correct.
   Definition correct_BUGEINT :
     forall n target,
     0 <= n -> Int.min_signed <= n <= Int.max_signed ->
     handler_correct (handle_BUGEINT n target) f_instr_BUGEINT
       (pre_and (pre_and (pre_and (pre_and code_ne_struct (code_at (Int.repr n))) (branch_offset_at target)) accu_unsigned_int) accu_is_long)
       (fun msg s => msg = "BUGEINT: not an integer"%string /\ match Machine.accu s with Val_int _ => False | _ => True end) (fun _ => False) (fun _ _ _ => False)
-    := verify_BUGEINT_handler_correct.
+    := BUGEINT_correct.verify_BUGEINT_handler_correct.
   Definition correct_BULTINT :
     forall n target,
     0 <= n -> Int.min_signed <= n <= Int.max_signed ->
     handler_correct (handle_BULTINT n target) f_instr_BULTINT
       (pre_and (pre_and (pre_and (pre_and code_ne_struct (code_at (Int.repr n))) (branch_offset_at target)) accu_unsigned_int) accu_is_long)
       (fun msg s => msg = "BULTINT: not an integer"%string /\ match Machine.accu s with Val_int _ => False | _ => True end) (fun _ => False) (fun _ _ _ => False)
-    := verify_BULTINT_handler_correct.
-  Definition correct_CHECK_SIGNALS := verify_CHECK_SIGNALS_correct.
-  Definition correct_CLOSUREREC := CLOSUREREC_correct_for_spec.
-  Definition correct_CLOSURE := CLOSURE_correct_for_spec.
-  Definition correct_CONST0 := verify_CONST0_compl_comp.
-  Definition correct_CONST1 := verify_CONST1_correct.
-  Definition correct_CONST2 := verify_CONST2_correct.
-  Definition correct_CONST3 := verify_CONST3_correct.
-  Definition correct_CONSTINT := verify_CONSTINT_handler_correct.
-  Definition correct_C_CALL1 prim_idx := verify_C_CALL1_correct prim_idx.
-  Definition correct_C_CALL2 prim_idx := verify_C_CALL2_correct prim_idx.
-  Definition correct_C_CALL3 prim_idx := verify_C_CALL3_correct prim_idx.
-  Definition correct_C_CALL4 prim_idx := verify_C_CALL4_correct prim_idx.
-  Definition correct_C_CALL5 prim_idx := verify_C_CALL5_correct prim_idx.
-  Definition correct_C_CALLN nargs prim_idx := verify_C_CALLN_correct nargs prim_idx.
-  Definition correct_DIVINT := verify_DIVINT_handler_correct.
-  Definition correct_ENVACC1 := verify_ENVACC1_with_pre.
-  Definition correct_ENVACC2 := verify_ENVACC2_with_pre.
-  Definition correct_ENVACC3 := verify_ENVACC3_with_pre.
-  Definition correct_ENVACC4 := verify_ENVACC4_with_pre.
-  Definition correct_ENVACC := ENVACC_correct_for_spec.
-  Definition correct_EQ := verify_EQ_handler_correct.
-  Definition correct_EVENT := verify_EVENT_correct.
-  Definition correct_GEINT := verify_GEINT_handler_correct.
-  Definition correct_GETBYTESCHAR := verify_GETBYTESCHAR_correct.
-  Definition correct_GETDYNMET := verify_GETDYNMET_correct.
-  Definition correct_GETFIELD0 := verify_GETFIELD0_with_pre.
-  Definition correct_GETFIELD1 := verify_GETFIELD1_with_pre.
-  Definition correct_GETFIELD2 := verify_GETFIELD2_with_pre.
-  Definition correct_GETFIELD3 := verify_GETFIELD3_with_pre.
-  Definition correct_GETFIELD := GETFIELD_correct_for_spec.
-  Definition correct_GETFLOATFIELD := verify_GETFLOATFIELD_correct.
-  Definition correct_GETGLOBALFIELD := verify_GETGLOBALFIELD_correct.
+    := BULTINT_correct.verify_BULTINT_handler_correct.
+  Definition correct_CHECK_SIGNALS := CHECK_SIGNALS_correct.verify_CHECK_SIGNALS_correct.
+  Definition correct_CLOSUREREC := CLOSUREREC_correct.CLOSUREREC_correct_for_spec.
+  Definition correct_CLOSURE := CLOSURE_correct.CLOSURE_correct_for_spec.
+  Definition correct_CONST0 := CONST0_correct.verify_CONST0_compl_comp.
+  Definition correct_CONST1 := CONST1_correct.verify_CONST1_correct.
+  Definition correct_CONST2 := CONST2_correct.verify_CONST2_correct.
+  Definition correct_CONST3 := CONST3_correct.verify_CONST3_correct.
+  Definition correct_CONSTINT := CONSTINT_correct.verify_CONSTINT_handler_correct.
+  Definition correct_C_CALL1 prim_idx := C_CALL1_correct.verify_C_CALL1_correct prim_idx.
+  Definition correct_C_CALL2 prim_idx := C_CALL2_correct.verify_C_CALL2_correct prim_idx.
+  Definition correct_C_CALL3 prim_idx := C_CALL3_correct.verify_C_CALL3_correct prim_idx.
+  Definition correct_C_CALL4 prim_idx := C_CALL4_correct.verify_C_CALL4_correct prim_idx.
+  Definition correct_C_CALL5 prim_idx := C_CALL5_correct.verify_C_CALL5_correct prim_idx.
+  Definition correct_C_CALLN nargs prim_idx := C_CALLN_correct.verify_C_CALLN_correct nargs prim_idx.
+  Definition correct_DIVINT := DIVINT_correct.verify_DIVINT_handler_correct.
+  Definition correct_ENVACC1 := ENVACC1_correct.verify_ENVACC1_with_pre.
+  Definition correct_ENVACC2 := ENVACC2_correct.verify_ENVACC2_with_pre.
+  Definition correct_ENVACC3 := ENVACC3_correct.verify_ENVACC3_with_pre.
+  Definition correct_ENVACC4 := ENVACC4_correct.verify_ENVACC4_with_pre.
+  Definition correct_ENVACC := ENVACC_correct.ENVACC_correct_for_spec.
+  Definition correct_EQ := EQ_correct.verify_EQ_handler_correct.
+  Definition correct_EVENT := EVENT_correct.verify_EVENT_correct.
+  Definition correct_GEINT := GEINT_correct.verify_GEINT_handler_correct.
+  Definition correct_GETBYTESCHAR := GETBYTESCHAR_correct.verify_GETBYTESCHAR_correct.
+  Definition correct_GETDYNMET := GETDYNMET_correct.verify_GETDYNMET_correct.
+  Definition correct_GETFIELD0 := GETFIELD0_correct.verify_GETFIELD0_with_pre.
+  Definition correct_GETFIELD1 := GETFIELD1_correct.verify_GETFIELD1_with_pre.
+  Definition correct_GETFIELD2 := GETFIELD2_correct.verify_GETFIELD2_with_pre.
+  Definition correct_GETFIELD3 := GETFIELD3_correct.verify_GETFIELD3_with_pre.
+  Definition correct_GETFIELD := GETFIELD_correct.GETFIELD_correct_for_spec.
+  Definition correct_GETFLOATFIELD := GETFLOATFIELD_correct.verify_GETFLOATFIELD_correct.
+  Definition correct_GETGLOBALFIELD := GETGLOBALFIELD_correct.verify_GETGLOBALFIELD_correct.
   Definition correct_GETGLOBAL :
     forall n,
     0 <= Z.of_nat n <= Int.max_signed ->
     handler_correct (handle_GETGLOBAL n) f_instr_GETGLOBAL
       (pre_and (code_at (Int.repr (Z.of_nat n))) (global_offset_safe n))
       (fun _ s => nth_error s.(Machine.global) n = None) (fun _ => False) (fun _ _ _ => False)
-    := verify_GETGLOBAL_handler_correct.
-  Definition correct_GETMETHOD := verify_GETMETHOD_correct.
-  Definition correct_GETPUBMET := verify_GETPUBMET_correct.
-  Definition correct_GETSTRINGCHAR := verify_GETSTRINGCHAR_correct.
-  Definition correct_GETVECTITEM := verify_GETVECTITEM_correct.
-  Definition correct_GRAB := verify_GRAB_correct.
-  Definition correct_GTINT := verify_GTINT_handler_correct.
-  Definition correct_ISINT := verify_ISINT_handler_correct.
-  Definition correct_LEINT := verify_LEINT_handler_correct.
-  Definition correct_LSLINT := verify_LSLINT_handler_correct.
-  Definition correct_LSRINT := verify_LSRINT_handler_correct.
-  Definition correct_LTINT := verify_LTINT_handler_correct.
-  Definition correct_MAKEBLOCK1 := MAKEBLOCK1_correct_for_spec.
-  Definition correct_MAKEBLOCK2 := MAKEBLOCK2_correct_for_spec.
-  Definition correct_MAKEBLOCK3 := MAKEBLOCK3_correct_for_spec.
-  Definition correct_MAKEBLOCK := verify_MAKEBLOCK_correct.
-  Definition correct_MAKEFLOATBLOCK := verify_MAKEFLOATBLOCK_correct.
-  Definition correct_MODINT := verify_MODINT_handler_correct.
-  Definition correct_MULINT := verify_MULINT_correct.
-  Definition correct_NEGINT := verify_NEGINT_compl_comp.
-  Definition correct_NEQ := verify_NEQ_handler_correct.
-  Definition correct_OFFSETCLOSURE0 := verify_OFFSETCLOSURE0_compl_comp.
-  Definition correct_OFFSETCLOSURE2 := verify_OFFSETCLOSURE2_compl_comp.
-  Definition correct_OFFSETCLOSUREM2 := verify_OFFSETCLOSUREM2_compl_comp.
-  Definition correct_OFFSETCLOSURE := verify_OFFSETCLOSURE_correct.
-  Definition correct_OFFSETINT := verify_OFFSETINT_handler_correct.
-  Definition correct_OFFSETREF := verify_OFFSETREF_correct.
-  Definition correct_ORINT := verify_ORINT_correct.
-  Definition correct_PERFORM := verify_PERFORM_correct.
-  Definition correct_POPTRAP := verify_POPTRAP_correct.
+    := GETGLOBAL_correct.verify_GETGLOBAL_handler_correct.
+  Definition correct_GETMETHOD := GETMETHOD_correct.verify_GETMETHOD_correct.
+  Definition correct_GETPUBMET := GETPUBMET_correct.verify_GETPUBMET_correct.
+  Definition correct_GETSTRINGCHAR := GETSTRINGCHAR_correct.verify_GETSTRINGCHAR_correct.
+  Definition correct_GETVECTITEM := GETVECTITEM_correct.verify_GETVECTITEM_correct.
+  Definition correct_GRAB := GRAB_correct.verify_GRAB_correct.
+  Definition correct_GTINT := GTINT_correct.verify_GTINT_handler_correct.
+  Definition correct_ISINT := ISINT_correct.verify_ISINT_handler_correct.
+  Definition correct_LEINT := LEINT_correct.verify_LEINT_handler_correct.
+  Definition correct_LSLINT := LSLINT_correct.verify_LSLINT_handler_correct.
+  Definition correct_LSRINT := LSRINT_correct.verify_LSRINT_handler_correct.
+  Definition correct_LTINT := LTINT_correct.verify_LTINT_handler_correct.
+  Definition correct_MAKEBLOCK1 := MAKEBLOCK1_correct.MAKEBLOCK1_correct_for_spec.
+  Definition correct_MAKEBLOCK2 := MAKEBLOCK2_correct.MAKEBLOCK2_correct_for_spec.
+  Definition correct_MAKEBLOCK3 := MAKEBLOCK3_correct.MAKEBLOCK3_correct_for_spec.
+  Definition correct_MAKEBLOCK := MAKEBLOCK_correct.verify_MAKEBLOCK_correct.
+  Definition correct_MAKEFLOATBLOCK := MAKEFLOATBLOCK_correct.verify_MAKEFLOATBLOCK_correct.
+  Definition correct_MODINT := MODINT_correct.verify_MODINT_handler_correct.
+  Definition correct_MULINT := MULINT_correct.verify_MULINT_correct.
+  Definition correct_NEGINT := NEGINT_correct.verify_NEGINT_compl_comp.
+  Definition correct_NEQ := NEQ_correct.verify_NEQ_handler_correct.
+  Definition correct_OFFSETCLOSURE0 := OFFSETCLOSURE0_correct.verify_OFFSETCLOSURE0_compl_comp.
+  Definition correct_OFFSETCLOSURE2 := OFFSETCLOSURE2_correct.verify_OFFSETCLOSURE2_compl_comp.
+  Definition correct_OFFSETCLOSUREM2 := OFFSETCLOSUREM2_correct.verify_OFFSETCLOSUREM2_compl_comp.
+  Definition correct_OFFSETCLOSURE := OFFSETCLOSURE_correct.verify_OFFSETCLOSURE_correct.
+  Definition correct_OFFSETINT := OFFSETINT_correct.verify_OFFSETINT_handler_correct.
+  Definition correct_OFFSETREF := OFFSETREF_correct.verify_OFFSETREF_correct.
+  Definition correct_ORINT := ORINT_correct.verify_ORINT_correct.
+  Definition correct_PERFORM := PERFORM_correct.verify_PERFORM_correct.
+  Definition correct_POPTRAP := POPTRAP_correct.verify_POPTRAP_correct.
   Definition correct_POP :
     forall n,
     Z.of_nat n < Int.half_modulus ->
     handler_correct (handle_POP n) f_instr_POP
       (pre_and (pre_and (code_at (Int.repr (Z.of_nat n))) code_ne_struct) (stack_length_ge n))
       (fun _ _ => False) (fun _ => False) (fun _ _ _ => False)
-    := verify_POP_handler_correct.
-  Definition correct_PUSHACC1 := verify_PUSHACC1_correct.
-  Definition correct_PUSHACC2 := verify_PUSHACC2_correct.
-  Definition correct_PUSHACC3 := verify_PUSHACC3_correct.
-  Definition correct_PUSHACC4 := verify_PUSHACC4_correct.
-  Definition correct_PUSHACC5 := verify_PUSHACC5_correct.
-  Definition correct_PUSHACC6 := verify_PUSHACC6_correct.
-  Definition correct_PUSHACC7 := verify_PUSHACC7_correct.
-  Definition correct_PUSHATOM0 := verify_PUSHATOM0_correct.
+    := POP_correct.verify_POP_handler_correct.
+  Definition correct_PUSHACC1 := PUSHACC1_correct.verify_PUSHACC1_correct.
+  Definition correct_PUSHACC2 := PUSHACC2_correct.verify_PUSHACC2_correct.
+  Definition correct_PUSHACC3 := PUSHACC3_correct.verify_PUSHACC3_correct.
+  Definition correct_PUSHACC4 := PUSHACC4_correct.verify_PUSHACC4_correct.
+  Definition correct_PUSHACC5 := PUSHACC5_correct.verify_PUSHACC5_correct.
+  Definition correct_PUSHACC6 := PUSHACC6_correct.verify_PUSHACC6_correct.
+  Definition correct_PUSHACC7 := PUSHACC7_correct.verify_PUSHACC7_correct.
+  Definition correct_PUSHATOM0 := PUSHATOM0_correct.verify_PUSHATOM0_correct.
   Definition correct_PUSHATOM :
     forall t, Z.of_nat t <= 2097151 ->
     handler_correct (handle_PUSHATOM t) f_instr_PUSHATOM
       (pre_and (sp_at_least 16) (code_at (Int.repr (Z.of_nat t))))
       (fun _ _ => False) (fun _ => False) (fun _ _ _ => False)
-    := verify_PUSHATOM_handler_correct.
-  Definition correct_PUSHCONST0 := verify_PUSHCONST0_correct.
-  Definition correct_PUSHCONST1 := verify_PUSHCONST1_correct.
-  Definition correct_PUSHCONST2 := verify_PUSHCONST2_correct.
-  Definition correct_PUSHCONST3 := verify_PUSHCONST3_correct.
-  Definition correct_PUSHCONSTINT := verify_PUSHCONSTINT_correct.
-  Definition correct_PUSHENVACC1 := verify_PUSHENVACC1_correct.
-  Definition correct_PUSHENVACC2 := verify_PUSHENVACC2_correct.
-  Definition correct_PUSHENVACC3 := verify_PUSHENVACC3_correct.
-  Definition correct_PUSHENVACC4 := verify_PUSHENVACC4_correct.
-  Definition correct_PUSHENVACC := verify_PUSHENVACC_correct.
-  Definition correct_PUSHGETGLOBALFIELD := verify_PUSHGETGLOBALFIELD_correct.
+    := PUSHATOM_correct.verify_PUSHATOM_handler_correct.
+  Definition correct_PUSHCONST0 := PUSHCONST0_correct.verify_PUSHCONST0_correct.
+  Definition correct_PUSHCONST1 := PUSHCONST1_correct.verify_PUSHCONST1_correct.
+  Definition correct_PUSHCONST2 := PUSHCONST2_correct.verify_PUSHCONST2_correct.
+  Definition correct_PUSHCONST3 := PUSHCONST3_correct.verify_PUSHCONST3_correct.
+  Definition correct_PUSHCONSTINT := PUSHCONSTINT_correct.verify_PUSHCONSTINT_correct.
+  Definition correct_PUSHENVACC1 := PUSHENVACC1_correct.verify_PUSHENVACC1_correct.
+  Definition correct_PUSHENVACC2 := PUSHENVACC2_correct.verify_PUSHENVACC2_correct.
+  Definition correct_PUSHENVACC3 := PUSHENVACC3_correct.verify_PUSHENVACC3_correct.
+  Definition correct_PUSHENVACC4 := PUSHENVACC4_correct.verify_PUSHENVACC4_correct.
+  Definition correct_PUSHENVACC := PUSHENVACC_correct.verify_PUSHENVACC_correct.
+  Definition correct_PUSHGETGLOBALFIELD := PUSHGETGLOBALFIELD_correct.verify_PUSHGETGLOBALFIELD_correct.
   Definition correct_PUSHGETGLOBAL :
     forall n,
     0 <= Z.of_nat n <= Int.max_signed ->
     handler_correct (handle_PUSHGETGLOBAL n) f_instr_PUSHGETGLOBAL
       (pre_and (pre_and (code_at (Int.repr (Z.of_nat n))) (global_offset_safe n)) (sp_at_least 16))
       (fun _ s => nth_error s.(Machine.global) n = None) (fun _ => False) (fun _ _ _ => False)
-    := verify_PUSHGETGLOBAL_handler_correct.
-  Definition correct_PUSHOFFSETCLOSURE0 := verify_PUSHOFFSETCLOSURE0_correct.
-  Definition correct_PUSHOFFSETCLOSURE2 := verify_PUSHOFFSETCLOSURE2_correct.
-  Definition correct_PUSHOFFSETCLOSUREM2 := verify_PUSHOFFSETCLOSUREM2_correct.
-  Definition correct_PUSHOFFSETCLOSURE := verify_PUSHOFFSETCLOSURE_correct.
-  Definition correct_PUSHTRAP := verify_PUSHTRAP_correct.
-  Definition correct_PUSH_RETADDR := verify_PUSH_RETADDR_correct.
-  Definition correct_PUSH := verify_PUSH_correct.
-  Definition correct_RAISE_NOTRACE := verify_RAISE_NOTRACE_correct.
-  Definition correct_RAISE := verify_RAISE_correct.
-  Definition correct_REPERFORMTERM := verify_REPERFORMTERM_correct.
-  Definition correct_RERAISE := verify_RERAISE_correct.
-  Definition correct_RESTART := verify_RESTART_correct.
-  Definition correct_RESUMETERM := verify_RESUMETERM_correct.
-  Definition correct_RESUME := verify_RESUME_correct.
-  Definition correct_RETURN := verify_RETURN_correct.
-  Definition correct_SETBYTESCHAR := verify_SETBYTESCHAR_correct.
-  Definition correct_SETFIELD0 := verify_SETFIELD0_correct.
-  Definition correct_SETFIELD1 := verify_SETFIELD1_correct.
-  Definition correct_SETFIELD2 := verify_SETFIELD2_correct.
-  Definition correct_SETFIELD3 := verify_SETFIELD3_correct.
-  Definition correct_SETFIELD := verify_SETFIELD_correct.
-  Definition correct_SETFLOATFIELD := verify_SETFLOATFIELD_correct.
-  Definition correct_SETGLOBAL := verify_SETGLOBAL_correct.
-  Definition correct_SETVECTITEM := verify_SETVECTITEM_correct.
-  Definition correct_STOP := verify_STOP_correct.
-  Definition correct_SUBINT := verify_SUBINT_correct.
-  Definition correct_SWITCH := verify_SWITCH_handler_correct.
-  Definition correct_UGEINT := verify_UGEINT_handler_correct.
-  Definition correct_ULTINT := verify_ULTINT_handler_correct.
-  Definition correct_VECTLENGTH := verify_VECTLENGTH_correct.
-  Definition correct_XORINT := verify_XORINT_correct.
+    := PUSHGETGLOBAL_correct.verify_PUSHGETGLOBAL_handler_correct.
+  Definition correct_PUSHOFFSETCLOSURE0 := PUSHOFFSETCLOSURE0_correct.verify_PUSHOFFSETCLOSURE0_correct.
+  Definition correct_PUSHOFFSETCLOSURE2 := PUSHOFFSETCLOSURE2_correct.verify_PUSHOFFSETCLOSURE2_correct.
+  Definition correct_PUSHOFFSETCLOSUREM2 := PUSHOFFSETCLOSUREM2_correct.verify_PUSHOFFSETCLOSUREM2_correct.
+  Definition correct_PUSHOFFSETCLOSURE := PUSHOFFSETCLOSURE_correct.verify_PUSHOFFSETCLOSURE_correct.
+  Definition correct_PUSHTRAP := PUSHTRAP_correct.verify_PUSHTRAP_correct.
+  Definition correct_PUSH_RETADDR := PUSH_RETADDR_correct.verify_PUSH_RETADDR_correct.
+  Definition correct_PUSH := PUSH_correct.verify_PUSH_correct.
+  Definition correct_RAISE_NOTRACE := RAISE_NOTRACE_correct.verify_RAISE_NOTRACE_correct.
+  Definition correct_RAISE := RAISE_correct.verify_RAISE_correct.
+  Definition correct_REPERFORMTERM := REPERFORMTERM_correct.verify_REPERFORMTERM_correct.
+  Definition correct_RERAISE := RERAISE_correct.verify_RERAISE_correct.
+  Definition correct_RESTART := RESTART_correct.verify_RESTART_correct.
+  Definition correct_RESUMETERM := RESUMETERM_correct.verify_RESUMETERM_correct.
+  Definition correct_RESUME := RESUME_correct.verify_RESUME_correct.
+  Definition correct_RETURN := RETURN_correct.verify_RETURN_correct.
+  Definition correct_SETBYTESCHAR := SETBYTESCHAR_correct.verify_SETBYTESCHAR_correct.
+  Definition correct_SETFIELD0 := SETFIELD0_correct.verify_SETFIELD0_correct.
+  Definition correct_SETFIELD1 := SETFIELD1_correct.verify_SETFIELD1_correct.
+  Definition correct_SETFIELD2 := SETFIELD2_correct.verify_SETFIELD2_correct.
+  Definition correct_SETFIELD3 := SETFIELD3_correct.verify_SETFIELD3_correct.
+  Definition correct_SETFIELD := SETFIELD_correct.verify_SETFIELD_correct.
+  Definition correct_SETFLOATFIELD := SETFLOATFIELD_correct.verify_SETFLOATFIELD_correct.
+  Definition correct_SETGLOBAL := SETGLOBAL_correct.verify_SETGLOBAL_correct.
+  Definition correct_SETVECTITEM := SETVECTITEM_correct.verify_SETVECTITEM_correct.
+  Definition correct_STOP := STOP_correct.verify_STOP_correct.
+  Definition correct_SUBINT := SUBINT_correct.verify_SUBINT_correct.
+  Definition correct_SWITCH := SWITCH_correct.verify_SWITCH_handler_correct.
+  Definition correct_UGEINT := UGEINT_correct.verify_UGEINT_handler_correct.
+  Definition correct_ULTINT := ULTINT_correct.verify_ULTINT_handler_correct.
+  Definition correct_VECTLENGTH := VECTLENGTH_correct.verify_VECTLENGTH_correct.
+  Definition correct_XORINT := XORINT_correct.verify_XORINT_correct.
+
+  Section __.
+  Set Printing All.
+  Set Printing Fully Qualified.
+  Set Printing Depth 10000000000.
+  Set Printing Width 2000.
+  Goal True.
+    idtac "<correct_ACC0>".
+    idtac "<PrintAssumptions>".
+    Print Assumptions correct_ACC0.
+    idtac "</PrintAssumptions>".
+    idtac "</correct_ACC0>".
+  Abort.
+  Goal True.
+    idtac "<correct_ACC1>".
+    idtac "<PrintAssumptions>".
+    Print Assumptions correct_ACC1.
+    idtac "</PrintAssumptions>".
+    idtac "</correct_ACC1>".
+  Abort.
+  Goal True.
+    idtac "<correct_ACC2>".
+    idtac "<PrintAssumptions>".
+    Print Assumptions correct_ACC2.
+    idtac "</PrintAssumptions>".
+    idtac "</correct_ACC2>".
+  Abort.
+  Goal True.
+    idtac "<correct_ACC3>".
+    idtac "<PrintAssumptions>".
+    Print Assumptions correct_ACC3.
+    idtac "</PrintAssumptions>".
+    idtac "</correct_ACC3>".
+  Abort.
+  Goal True.
+    idtac "<correct_ACC4>".
+    idtac "<PrintAssumptions>".
+    Print Assumptions correct_ACC4.
+    idtac "</PrintAssumptions>".
+    idtac "</correct_ACC4>".
+  Abort.
+  Goal True.
+    idtac "<correct_ACC5>".
+    idtac "<PrintAssumptions>".
+    Print Assumptions correct_ACC5.
+    idtac "</PrintAssumptions>".
+    idtac "</correct_ACC5>".
+  Abort.
+  Goal True.
+    idtac "<correct_ACC6>".
+    idtac "<PrintAssumptions>".
+    Print Assumptions correct_ACC6.
+    idtac "</PrintAssumptions>".
+    idtac "</correct_ACC6>".
+  Abort.
+  Goal True.
+    idtac "<correct_ACC7>".
+    idtac "<PrintAssumptions>".
+    Print Assumptions correct_ACC7.
+    idtac "</PrintAssumptions>".
+    idtac "</correct_ACC7>".
+  Abort.
+  Goal True.
+    idtac "<correct_ACC>".
+    idtac "<PrintAssumptions>".
+    Print Assumptions correct_ACC.
+    idtac "</PrintAssumptions>".
+    idtac "</correct_ACC>".
+  Abort.
+  Goal True.
+    idtac "<correct_ADDINT>".
+    idtac "<PrintAssumptions>".
+    Print Assumptions correct_ADDINT.
+    idtac "</PrintAssumptions>".
+    idtac "</correct_ADDINT>".
+  Abort.
+  Goal True.
+    idtac "<correct_ANDINT>".
+    idtac "<PrintAssumptions>".
+    Print Assumptions correct_ANDINT.
+    idtac "</PrintAssumptions>".
+    idtac "</correct_ANDINT>".
+  Abort.
+  Goal True.
+    idtac "<correct_APPLY1>".
+    idtac "<PrintAssumptions>".
+    Print Assumptions correct_APPLY1.
+    idtac "</PrintAssumptions>".
+    idtac "</correct_APPLY1>".
+  Abort.
+  Goal True.
+    idtac "<correct_APPLY2>".
+    idtac "<PrintAssumptions>".
+    Print Assumptions correct_APPLY2.
+    idtac "</PrintAssumptions>".
+    idtac "</correct_APPLY2>".
+  Abort.
+  Goal True.
+    idtac "<correct_APPLY3>".
+    idtac "<PrintAssumptions>".
+    Print Assumptions correct_APPLY3.
+    idtac "</PrintAssumptions>".
+    idtac "</correct_APPLY3>".
+  Abort.
+  Goal True.
+    idtac "<correct_APPLY>".
+    idtac "<PrintAssumptions>".
+    Print Assumptions correct_APPLY.
+    idtac "</PrintAssumptions>".
+    idtac "</correct_APPLY>".
+  Abort.
+  Goal True.
+    idtac "<correct_APPTERM1>".
+    idtac "<PrintAssumptions>".
+    Print Assumptions correct_APPTERM1.
+    idtac "</PrintAssumptions>".
+    idtac "</correct_APPTERM1>".
+  Abort.
+  Goal True.
+    idtac "<correct_APPTERM2>".
+    idtac "<PrintAssumptions>".
+    Print Assumptions correct_APPTERM2.
+    idtac "</PrintAssumptions>".
+    idtac "</correct_APPTERM2>".
+  Abort.
+  Goal True.
+    idtac "<correct_APPTERM3>".
+    idtac "<PrintAssumptions>".
+    Print Assumptions correct_APPTERM3.
+    idtac "</PrintAssumptions>".
+    idtac "</correct_APPTERM3>".
+  Abort.
+  Goal True.
+    idtac "<correct_APPTERM>".
+    idtac "<PrintAssumptions>".
+    Print Assumptions correct_APPTERM.
+    idtac "</PrintAssumptions>".
+    idtac "</correct_APPTERM>".
+  Abort.
+  Goal True.
+    idtac "<correct_ASRINT>".
+    idtac "<PrintAssumptions>".
+    Print Assumptions correct_ASRINT.
+    idtac "</PrintAssumptions>".
+    idtac "</correct_ASRINT>".
+  Abort.
+  Goal True.
+    idtac "<correct_ASSIGN>".
+    idtac "<PrintAssumptions>".
+    Print Assumptions correct_ASSIGN.
+    idtac "</PrintAssumptions>".
+    idtac "</correct_ASSIGN>".
+  Abort.
+  Goal True.
+    idtac "<correct_ATOM0>".
+    idtac "<PrintAssumptions>".
+    Print Assumptions correct_ATOM0.
+    idtac "</PrintAssumptions>".
+    idtac "</correct_ATOM0>".
+  Abort.
+  Goal True.
+    idtac "<correct_ATOM>".
+    idtac "<PrintAssumptions>".
+    Print Assumptions correct_ATOM.
+    idtac "</PrintAssumptions>".
+    idtac "</correct_ATOM>".
+  Abort.
+  Goal True.
+    idtac "<correct_BEQ>".
+    idtac "<PrintAssumptions>".
+    Print Assumptions correct_BEQ.
+    idtac "</PrintAssumptions>".
+    idtac "</correct_BEQ>".
+  Abort.
+  Goal True.
+    idtac "<correct_BGEINT>".
+    idtac "<PrintAssumptions>".
+    Print Assumptions correct_BGEINT.
+    idtac "</PrintAssumptions>".
+    idtac "</correct_BGEINT>".
+  Abort.
+  Goal True.
+    idtac "<correct_BGTINT>".
+    idtac "<PrintAssumptions>".
+    Print Assumptions correct_BGTINT.
+    idtac "</PrintAssumptions>".
+    idtac "</correct_BGTINT>".
+  Abort.
+  Goal True.
+    idtac "<correct_BLEINT>".
+    idtac "<PrintAssumptions>".
+    Print Assumptions correct_BLEINT.
+    idtac "</PrintAssumptions>".
+    idtac "</correct_BLEINT>".
+  Abort.
+  Goal True.
+    idtac "<correct_BLTINT>".
+    idtac "<PrintAssumptions>".
+    Print Assumptions correct_BLTINT.
+    idtac "</PrintAssumptions>".
+    idtac "</correct_BLTINT>".
+  Abort.
+  Goal True.
+    idtac "<correct_BNEQ>".
+    idtac "<PrintAssumptions>".
+    Print Assumptions correct_BNEQ.
+    idtac "</PrintAssumptions>".
+    idtac "</correct_BNEQ>".
+  Abort.
+  Goal True.
+    idtac "<correct_BOOLNOT>".
+    idtac "<PrintAssumptions>".
+    Print Assumptions correct_BOOLNOT.
+    idtac "</PrintAssumptions>".
+    idtac "</correct_BOOLNOT>".
+  Abort.
+  Goal True.
+    idtac "<correct_BRANCHIFNOT>".
+    idtac "<PrintAssumptions>".
+    Print Assumptions correct_BRANCHIFNOT.
+    idtac "</PrintAssumptions>".
+    idtac "</correct_BRANCHIFNOT>".
+  Abort.
+  Goal True.
+    idtac "<correct_BRANCHIF>".
+    idtac "<PrintAssumptions>".
+    Print Assumptions correct_BRANCHIF.
+    idtac "</PrintAssumptions>".
+    idtac "</correct_BRANCHIF>".
+  Abort.
+  Goal True.
+    idtac "<correct_BRANCH>".
+    idtac "<PrintAssumptions>".
+    Print Assumptions correct_BRANCH.
+    idtac "</PrintAssumptions>".
+    idtac "</correct_BRANCH>".
+  Abort.
+  Goal True.
+    idtac "<correct_BREAK>".
+    idtac "<PrintAssumptions>".
+    Print Assumptions correct_BREAK.
+    idtac "</PrintAssumptions>".
+    idtac "</correct_BREAK>".
+  Abort.
+  Goal True.
+    idtac "<correct_BUGEINT>".
+    idtac "<PrintAssumptions>".
+    Print Assumptions correct_BUGEINT.
+    idtac "</PrintAssumptions>".
+    idtac "</correct_BUGEINT>".
+  Abort.
+  Goal True.
+    idtac "<correct_BULTINT>".
+    idtac "<PrintAssumptions>".
+    Print Assumptions correct_BULTINT.
+    idtac "</PrintAssumptions>".
+    idtac "</correct_BULTINT>".
+  Abort.
+  Goal True.
+    idtac "<correct_CHECK_SIGNALS>".
+    idtac "<PrintAssumptions>".
+    Print Assumptions correct_CHECK_SIGNALS.
+    idtac "</PrintAssumptions>".
+    idtac "</correct_CHECK_SIGNALS>".
+  Abort.
+  Goal True.
+    idtac "<correct_CLOSUREREC>".
+    idtac "<PrintAssumptions>".
+    Print Assumptions correct_CLOSUREREC.
+    idtac "</PrintAssumptions>".
+    idtac "</correct_CLOSUREREC>".
+  Abort.
+  Goal True.
+    idtac "<correct_CLOSURE>".
+    idtac "<PrintAssumptions>".
+    Print Assumptions correct_CLOSURE.
+    idtac "</PrintAssumptions>".
+    idtac "</correct_CLOSURE>".
+  Abort.
+  Goal True.
+    idtac "<correct_CONST0>".
+    idtac "<PrintAssumptions>".
+    Print Assumptions correct_CONST0.
+    idtac "</PrintAssumptions>".
+    idtac "</correct_CONST0>".
+  Abort.
+  Goal True.
+    idtac "<correct_CONST1>".
+    idtac "<PrintAssumptions>".
+    Print Assumptions correct_CONST1.
+    idtac "</PrintAssumptions>".
+    idtac "</correct_CONST1>".
+  Abort.
+  Goal True.
+    idtac "<correct_CONST2>".
+    idtac "<PrintAssumptions>".
+    Print Assumptions correct_CONST2.
+    idtac "</PrintAssumptions>".
+    idtac "</correct_CONST2>".
+  Abort.
+  Goal True.
+    idtac "<correct_CONST3>".
+    idtac "<PrintAssumptions>".
+    Print Assumptions correct_CONST3.
+    idtac "</PrintAssumptions>".
+    idtac "</correct_CONST3>".
+  Abort.
+  Goal True.
+    idtac "<correct_CONSTINT>".
+    idtac "<PrintAssumptions>".
+    Print Assumptions correct_CONSTINT.
+    idtac "</PrintAssumptions>".
+    idtac "</correct_CONSTINT>".
+  Abort.
+  Goal True.
+    idtac "<correct_C_CALL1>".
+    idtac "<PrintAssumptions>".
+    Print Assumptions correct_C_CALL1.
+    idtac "</PrintAssumptions>".
+    idtac "</correct_C_CALL1>".
+  Abort.
+  Goal True.
+    idtac "<correct_C_CALL2>".
+    idtac "<PrintAssumptions>".
+    Print Assumptions correct_C_CALL2.
+    idtac "</PrintAssumptions>".
+    idtac "</correct_C_CALL2>".
+  Abort.
+  Goal True.
+    idtac "<correct_C_CALL3>".
+    idtac "<PrintAssumptions>".
+    Print Assumptions correct_C_CALL3.
+    idtac "</PrintAssumptions>".
+    idtac "</correct_C_CALL3>".
+  Abort.
+  Goal True.
+    idtac "<correct_C_CALL4>".
+    idtac "<PrintAssumptions>".
+    Print Assumptions correct_C_CALL4.
+    idtac "</PrintAssumptions>".
+    idtac "</correct_C_CALL4>".
+  Abort.
+  Goal True.
+    idtac "<correct_C_CALL5>".
+    idtac "<PrintAssumptions>".
+    Print Assumptions correct_C_CALL5.
+    idtac "</PrintAssumptions>".
+    idtac "</correct_C_CALL5>".
+  Abort.
+  Goal True.
+    idtac "<correct_C_CALLN>".
+    idtac "<PrintAssumptions>".
+    Print Assumptions correct_C_CALLN.
+    idtac "</PrintAssumptions>".
+    idtac "</correct_C_CALLN>".
+  Abort.
+  Goal True.
+    idtac "<correct_DIVINT>".
+    idtac "<PrintAssumptions>".
+    Print Assumptions correct_DIVINT.
+    idtac "</PrintAssumptions>".
+    idtac "</correct_DIVINT>".
+  Abort.
+  Goal True.
+    idtac "<correct_ENVACC1>".
+    idtac "<PrintAssumptions>".
+    Print Assumptions correct_ENVACC1.
+    idtac "</PrintAssumptions>".
+    idtac "</correct_ENVACC1>".
+  Abort.
+  Goal True.
+    idtac "<correct_ENVACC2>".
+    idtac "<PrintAssumptions>".
+    Print Assumptions correct_ENVACC2.
+    idtac "</PrintAssumptions>".
+    idtac "</correct_ENVACC2>".
+  Abort.
+  Goal True.
+    idtac "<correct_ENVACC3>".
+    idtac "<PrintAssumptions>".
+    Print Assumptions correct_ENVACC3.
+    idtac "</PrintAssumptions>".
+    idtac "</correct_ENVACC3>".
+  Abort.
+  Goal True.
+    idtac "<correct_ENVACC4>".
+    idtac "<PrintAssumptions>".
+    Print Assumptions correct_ENVACC4.
+    idtac "</PrintAssumptions>".
+    idtac "</correct_ENVACC4>".
+  Abort.
+  Goal True.
+    idtac "<correct_ENVACC>".
+    idtac "<PrintAssumptions>".
+    Print Assumptions correct_ENVACC.
+    idtac "</PrintAssumptions>".
+    idtac "</correct_ENVACC>".
+  Abort.
+  Goal True.
+    idtac "<correct_EQ>".
+    idtac "<PrintAssumptions>".
+    Print Assumptions correct_EQ.
+    idtac "</PrintAssumptions>".
+    idtac "</correct_EQ>".
+  Abort.
+  Goal True.
+    idtac "<correct_EVENT>".
+    idtac "<PrintAssumptions>".
+    Print Assumptions correct_EVENT.
+    idtac "</PrintAssumptions>".
+    idtac "</correct_EVENT>".
+  Abort.
+  Goal True.
+    idtac "<correct_GEINT>".
+    idtac "<PrintAssumptions>".
+    Print Assumptions correct_GEINT.
+    idtac "</PrintAssumptions>".
+    idtac "</correct_GEINT>".
+  Abort.
+  Goal True.
+    idtac "<correct_GETBYTESCHAR>".
+    idtac "<PrintAssumptions>".
+    Print Assumptions correct_GETBYTESCHAR.
+    idtac "</PrintAssumptions>".
+    idtac "</correct_GETBYTESCHAR>".
+  Abort.
+  Goal True.
+    idtac "<correct_GETDYNMET>".
+    idtac "<PrintAssumptions>".
+    Print Assumptions correct_GETDYNMET.
+    idtac "</PrintAssumptions>".
+    idtac "</correct_GETDYNMET>".
+  Abort.
+  Goal True.
+    idtac "<correct_GETFIELD0>".
+    idtac "<PrintAssumptions>".
+    Print Assumptions correct_GETFIELD0.
+    idtac "</PrintAssumptions>".
+    idtac "</correct_GETFIELD0>".
+  Abort.
+  Goal True.
+    idtac "<correct_GETFIELD1>".
+    idtac "<PrintAssumptions>".
+    Print Assumptions correct_GETFIELD1.
+    idtac "</PrintAssumptions>".
+    idtac "</correct_GETFIELD1>".
+  Abort.
+  Goal True.
+    idtac "<correct_GETFIELD2>".
+    idtac "<PrintAssumptions>".
+    Print Assumptions correct_GETFIELD2.
+    idtac "</PrintAssumptions>".
+    idtac "</correct_GETFIELD2>".
+  Abort.
+  Goal True.
+    idtac "<correct_GETFIELD3>".
+    idtac "<PrintAssumptions>".
+    Print Assumptions correct_GETFIELD3.
+    idtac "</PrintAssumptions>".
+    idtac "</correct_GETFIELD3>".
+  Abort.
+  Goal True.
+    idtac "<correct_GETFIELD>".
+    idtac "<PrintAssumptions>".
+    Print Assumptions correct_GETFIELD.
+    idtac "</PrintAssumptions>".
+    idtac "</correct_GETFIELD>".
+  Abort.
+  Goal True.
+    idtac "<correct_GETFLOATFIELD>".
+    idtac "<PrintAssumptions>".
+    Print Assumptions correct_GETFLOATFIELD.
+    idtac "</PrintAssumptions>".
+    idtac "</correct_GETFLOATFIELD>".
+  Abort.
+  Goal True.
+    idtac "<correct_GETGLOBALFIELD>".
+    idtac "<PrintAssumptions>".
+    Print Assumptions correct_GETGLOBALFIELD.
+    idtac "</PrintAssumptions>".
+    idtac "</correct_GETGLOBALFIELD>".
+  Abort.
+  Goal True.
+    idtac "<correct_GETGLOBAL>".
+    idtac "<PrintAssumptions>".
+    Print Assumptions correct_GETGLOBAL.
+    idtac "</PrintAssumptions>".
+    idtac "</correct_GETGLOBAL>".
+  Abort.
+  Goal True.
+    idtac "<correct_GETMETHOD>".
+    idtac "<PrintAssumptions>".
+    Print Assumptions correct_GETMETHOD.
+    idtac "</PrintAssumptions>".
+    idtac "</correct_GETMETHOD>".
+  Abort.
+  Goal True.
+    idtac "<correct_GETPUBMET>".
+    idtac "<PrintAssumptions>".
+    Print Assumptions correct_GETPUBMET.
+    idtac "</PrintAssumptions>".
+    idtac "</correct_GETPUBMET>".
+  Abort.
+  Goal True.
+    idtac "<correct_GETSTRINGCHAR>".
+    idtac "<PrintAssumptions>".
+    Print Assumptions correct_GETSTRINGCHAR.
+    idtac "</PrintAssumptions>".
+    idtac "</correct_GETSTRINGCHAR>".
+  Abort.
+  Goal True.
+    idtac "<correct_GETVECTITEM>".
+    idtac "<PrintAssumptions>".
+    Print Assumptions correct_GETVECTITEM.
+    idtac "</PrintAssumptions>".
+    idtac "</correct_GETVECTITEM>".
+  Abort.
+  Goal True.
+    idtac "<correct_GRAB>".
+    idtac "<PrintAssumptions>".
+    Print Assumptions correct_GRAB.
+    idtac "</PrintAssumptions>".
+    idtac "</correct_GRAB>".
+  Abort.
+  Goal True.
+    idtac "<correct_GTINT>".
+    idtac "<PrintAssumptions>".
+    Print Assumptions correct_GTINT.
+    idtac "</PrintAssumptions>".
+    idtac "</correct_GTINT>".
+  Abort.
+  Goal True.
+    idtac "<correct_ISINT>".
+    idtac "<PrintAssumptions>".
+    Print Assumptions correct_ISINT.
+    idtac "</PrintAssumptions>".
+    idtac "</correct_ISINT>".
+  Abort.
+  Goal True.
+    idtac "<correct_LEINT>".
+    idtac "<PrintAssumptions>".
+    Print Assumptions correct_LEINT.
+    idtac "</PrintAssumptions>".
+    idtac "</correct_LEINT>".
+  Abort.
+  Goal True.
+    idtac "<correct_LSLINT>".
+    idtac "<PrintAssumptions>".
+    Print Assumptions correct_LSLINT.
+    idtac "</PrintAssumptions>".
+    idtac "</correct_LSLINT>".
+  Abort.
+  Goal True.
+    idtac "<correct_LSRINT>".
+    idtac "<PrintAssumptions>".
+    Print Assumptions correct_LSRINT.
+    idtac "</PrintAssumptions>".
+    idtac "</correct_LSRINT>".
+  Abort.
+  Goal True.
+    idtac "<correct_LTINT>".
+    idtac "<PrintAssumptions>".
+    Print Assumptions correct_LTINT.
+    idtac "</PrintAssumptions>".
+    idtac "</correct_LTINT>".
+  Abort.
+  Goal True.
+    idtac "<correct_MAKEBLOCK1>".
+    idtac "<PrintAssumptions>".
+    Print Assumptions correct_MAKEBLOCK1.
+    idtac "</PrintAssumptions>".
+    idtac "</correct_MAKEBLOCK1>".
+  Abort.
+  Goal True.
+    idtac "<correct_MAKEBLOCK2>".
+    idtac "<PrintAssumptions>".
+    Print Assumptions correct_MAKEBLOCK2.
+    idtac "</PrintAssumptions>".
+    idtac "</correct_MAKEBLOCK2>".
+  Abort.
+  Goal True.
+    idtac "<correct_MAKEBLOCK3>".
+    idtac "<PrintAssumptions>".
+    Print Assumptions correct_MAKEBLOCK3.
+    idtac "</PrintAssumptions>".
+    idtac "</correct_MAKEBLOCK3>".
+  Abort.
+  Goal True.
+    idtac "<correct_MAKEBLOCK>".
+    idtac "<PrintAssumptions>".
+    Print Assumptions correct_MAKEBLOCK.
+    idtac "</PrintAssumptions>".
+    idtac "</correct_MAKEBLOCK>".
+  Abort.
+  Goal True.
+    idtac "<correct_MAKEFLOATBLOCK>".
+    idtac "<PrintAssumptions>".
+    Print Assumptions correct_MAKEFLOATBLOCK.
+    idtac "</PrintAssumptions>".
+    idtac "</correct_MAKEFLOATBLOCK>".
+  Abort.
+  Goal True.
+    idtac "<correct_MODINT>".
+    idtac "<PrintAssumptions>".
+    Print Assumptions correct_MODINT.
+    idtac "</PrintAssumptions>".
+    idtac "</correct_MODINT>".
+  Abort.
+  Goal True.
+    idtac "<correct_MULINT>".
+    idtac "<PrintAssumptions>".
+    Print Assumptions correct_MULINT.
+    idtac "</PrintAssumptions>".
+    idtac "</correct_MULINT>".
+  Abort.
+  Goal True.
+    idtac "<correct_NEGINT>".
+    idtac "<PrintAssumptions>".
+    Print Assumptions correct_NEGINT.
+    idtac "</PrintAssumptions>".
+    idtac "</correct_NEGINT>".
+  Abort.
+  Goal True.
+    idtac "<correct_NEQ>".
+    idtac "<PrintAssumptions>".
+    Print Assumptions correct_NEQ.
+    idtac "</PrintAssumptions>".
+    idtac "</correct_NEQ>".
+  Abort.
+  Goal True.
+    idtac "<correct_OFFSETCLOSURE0>".
+    idtac "<PrintAssumptions>".
+    Print Assumptions correct_OFFSETCLOSURE0.
+    idtac "</PrintAssumptions>".
+    idtac "</correct_OFFSETCLOSURE0>".
+  Abort.
+  Goal True.
+    idtac "<correct_OFFSETCLOSURE2>".
+    idtac "<PrintAssumptions>".
+    Print Assumptions correct_OFFSETCLOSURE2.
+    idtac "</PrintAssumptions>".
+    idtac "</correct_OFFSETCLOSURE2>".
+  Abort.
+  Goal True.
+    idtac "<correct_OFFSETCLOSUREM2>".
+    idtac "<PrintAssumptions>".
+    Print Assumptions correct_OFFSETCLOSUREM2.
+    idtac "</PrintAssumptions>".
+    idtac "</correct_OFFSETCLOSUREM2>".
+  Abort.
+  Goal True.
+    idtac "<correct_OFFSETCLOSURE>".
+    idtac "<PrintAssumptions>".
+    Print Assumptions correct_OFFSETCLOSURE.
+    idtac "</PrintAssumptions>".
+    idtac "</correct_OFFSETCLOSURE>".
+  Abort.
+  Goal True.
+    idtac "<correct_OFFSETINT>".
+    idtac "<PrintAssumptions>".
+    Print Assumptions correct_OFFSETINT.
+    idtac "</PrintAssumptions>".
+    idtac "</correct_OFFSETINT>".
+  Abort.
+  Goal True.
+    idtac "<correct_OFFSETREF>".
+    idtac "<PrintAssumptions>".
+    Print Assumptions correct_OFFSETREF.
+    idtac "</PrintAssumptions>".
+    idtac "</correct_OFFSETREF>".
+  Abort.
+  Goal True.
+    idtac "<correct_ORINT>".
+    idtac "<PrintAssumptions>".
+    Print Assumptions correct_ORINT.
+    idtac "</PrintAssumptions>".
+    idtac "</correct_ORINT>".
+  Abort.
+  Goal True.
+    idtac "<correct_PERFORM>".
+    idtac "<PrintAssumptions>".
+    Print Assumptions correct_PERFORM.
+    idtac "</PrintAssumptions>".
+    idtac "</correct_PERFORM>".
+  Abort.
+  Goal True.
+    idtac "<correct_POPTRAP>".
+    idtac "<PrintAssumptions>".
+    Print Assumptions correct_POPTRAP.
+    idtac "</PrintAssumptions>".
+    idtac "</correct_POPTRAP>".
+  Abort.
+  Goal True.
+    idtac "<correct_POP>".
+    idtac "<PrintAssumptions>".
+    Print Assumptions correct_POP.
+    idtac "</PrintAssumptions>".
+    idtac "</correct_POP>".
+  Abort.
+  Goal True.
+    idtac "<correct_PUSHACC1>".
+    idtac "<PrintAssumptions>".
+    Print Assumptions correct_PUSHACC1.
+    idtac "</PrintAssumptions>".
+    idtac "</correct_PUSHACC1>".
+  Abort.
+  Goal True.
+    idtac "<correct_PUSHACC2>".
+    idtac "<PrintAssumptions>".
+    Print Assumptions correct_PUSHACC2.
+    idtac "</PrintAssumptions>".
+    idtac "</correct_PUSHACC2>".
+  Abort.
+  Goal True.
+    idtac "<correct_PUSHACC3>".
+    idtac "<PrintAssumptions>".
+    Print Assumptions correct_PUSHACC3.
+    idtac "</PrintAssumptions>".
+    idtac "</correct_PUSHACC3>".
+  Abort.
+  Goal True.
+    idtac "<correct_PUSHACC4>".
+    idtac "<PrintAssumptions>".
+    Print Assumptions correct_PUSHACC4.
+    idtac "</PrintAssumptions>".
+    idtac "</correct_PUSHACC4>".
+  Abort.
+  Goal True.
+    idtac "<correct_PUSHACC5>".
+    idtac "<PrintAssumptions>".
+    Print Assumptions correct_PUSHACC5.
+    idtac "</PrintAssumptions>".
+    idtac "</correct_PUSHACC5>".
+  Abort.
+  Goal True.
+    idtac "<correct_PUSHACC6>".
+    idtac "<PrintAssumptions>".
+    Print Assumptions correct_PUSHACC6.
+    idtac "</PrintAssumptions>".
+    idtac "</correct_PUSHACC6>".
+  Abort.
+  Goal True.
+    idtac "<correct_PUSHACC7>".
+    idtac "<PrintAssumptions>".
+    Print Assumptions correct_PUSHACC7.
+    idtac "</PrintAssumptions>".
+    idtac "</correct_PUSHACC7>".
+  Abort.
+  Goal True.
+    idtac "<correct_PUSHATOM0>".
+    idtac "<PrintAssumptions>".
+    Print Assumptions correct_PUSHATOM0.
+    idtac "</PrintAssumptions>".
+    idtac "</correct_PUSHATOM0>".
+  Abort.
+  Goal True.
+    idtac "<correct_PUSHATOM>".
+    idtac "<PrintAssumptions>".
+    Print Assumptions correct_PUSHATOM.
+    idtac "</PrintAssumptions>".
+    idtac "</correct_PUSHATOM>".
+  Abort.
+  Goal True.
+    idtac "<correct_PUSHCONST0>".
+    idtac "<PrintAssumptions>".
+    Print Assumptions correct_PUSHCONST0.
+    idtac "</PrintAssumptions>".
+    idtac "</correct_PUSHCONST0>".
+  Abort.
+  Goal True.
+    idtac "<correct_PUSHCONST1>".
+    idtac "<PrintAssumptions>".
+    Print Assumptions correct_PUSHCONST1.
+    idtac "</PrintAssumptions>".
+    idtac "</correct_PUSHCONST1>".
+  Abort.
+  Goal True.
+    idtac "<correct_PUSHCONST2>".
+    idtac "<PrintAssumptions>".
+    Print Assumptions correct_PUSHCONST2.
+    idtac "</PrintAssumptions>".
+    idtac "</correct_PUSHCONST2>".
+  Abort.
+  Goal True.
+    idtac "<correct_PUSHCONST3>".
+    idtac "<PrintAssumptions>".
+    Print Assumptions correct_PUSHCONST3.
+    idtac "</PrintAssumptions>".
+    idtac "</correct_PUSHCONST3>".
+  Abort.
+  Goal True.
+    idtac "<correct_PUSHCONSTINT>".
+    idtac "<PrintAssumptions>".
+    Print Assumptions correct_PUSHCONSTINT.
+    idtac "</PrintAssumptions>".
+    idtac "</correct_PUSHCONSTINT>".
+  Abort.
+  Goal True.
+    idtac "<correct_PUSHENVACC1>".
+    idtac "<PrintAssumptions>".
+    Print Assumptions correct_PUSHENVACC1.
+    idtac "</PrintAssumptions>".
+    idtac "</correct_PUSHENVACC1>".
+  Abort.
+  Goal True.
+    idtac "<correct_PUSHENVACC2>".
+    idtac "<PrintAssumptions>".
+    Print Assumptions correct_PUSHENVACC2.
+    idtac "</PrintAssumptions>".
+    idtac "</correct_PUSHENVACC2>".
+  Abort.
+  Goal True.
+    idtac "<correct_PUSHENVACC3>".
+    idtac "<PrintAssumptions>".
+    Print Assumptions correct_PUSHENVACC3.
+    idtac "</PrintAssumptions>".
+    idtac "</correct_PUSHENVACC3>".
+  Abort.
+  Goal True.
+    idtac "<correct_PUSHENVACC4>".
+    idtac "<PrintAssumptions>".
+    Print Assumptions correct_PUSHENVACC4.
+    idtac "</PrintAssumptions>".
+    idtac "</correct_PUSHENVACC4>".
+  Abort.
+  Goal True.
+    idtac "<correct_PUSHENVACC>".
+    idtac "<PrintAssumptions>".
+    Print Assumptions correct_PUSHENVACC.
+    idtac "</PrintAssumptions>".
+    idtac "</correct_PUSHENVACC>".
+  Abort.
+  Goal True.
+    idtac "<correct_PUSHGETGLOBALFIELD>".
+    idtac "<PrintAssumptions>".
+    Print Assumptions correct_PUSHGETGLOBALFIELD.
+    idtac "</PrintAssumptions>".
+    idtac "</correct_PUSHGETGLOBALFIELD>".
+  Abort.
+  Goal True.
+    idtac "<correct_PUSHGETGLOBAL>".
+    idtac "<PrintAssumptions>".
+    Print Assumptions correct_PUSHGETGLOBAL.
+    idtac "</PrintAssumptions>".
+    idtac "</correct_PUSHGETGLOBAL>".
+  Abort.
+  Goal True.
+    idtac "<correct_PUSHOFFSETCLOSURE0>".
+    idtac "<PrintAssumptions>".
+    Print Assumptions correct_PUSHOFFSETCLOSURE0.
+    idtac "</PrintAssumptions>".
+    idtac "</correct_PUSHOFFSETCLOSURE0>".
+  Abort.
+  Goal True.
+    idtac "<correct_PUSHOFFSETCLOSURE2>".
+    idtac "<PrintAssumptions>".
+    Print Assumptions correct_PUSHOFFSETCLOSURE2.
+    idtac "</PrintAssumptions>".
+    idtac "</correct_PUSHOFFSETCLOSURE2>".
+  Abort.
+  Goal True.
+    idtac "<correct_PUSHOFFSETCLOSUREM2>".
+    idtac "<PrintAssumptions>".
+    Print Assumptions correct_PUSHOFFSETCLOSUREM2.
+    idtac "</PrintAssumptions>".
+    idtac "</correct_PUSHOFFSETCLOSUREM2>".
+  Abort.
+  Goal True.
+    idtac "<correct_PUSHOFFSETCLOSURE>".
+    idtac "<PrintAssumptions>".
+    Print Assumptions correct_PUSHOFFSETCLOSURE.
+    idtac "</PrintAssumptions>".
+    idtac "</correct_PUSHOFFSETCLOSURE>".
+  Abort.
+  Goal True.
+    idtac "<correct_PUSHTRAP>".
+    idtac "<PrintAssumptions>".
+    Print Assumptions correct_PUSHTRAP.
+    idtac "</PrintAssumptions>".
+    idtac "</correct_PUSHTRAP>".
+  Abort.
+  Goal True.
+    idtac "<correct_PUSH_RETADDR>".
+    idtac "<PrintAssumptions>".
+    Print Assumptions correct_PUSH_RETADDR.
+    idtac "</PrintAssumptions>".
+    idtac "</correct_PUSH_RETADDR>".
+  Abort.
+  Goal True.
+    idtac "<correct_PUSH>".
+    idtac "<PrintAssumptions>".
+    Print Assumptions correct_PUSH.
+    idtac "</PrintAssumptions>".
+    idtac "</correct_PUSH>".
+  Abort.
+  Goal True.
+    idtac "<correct_RAISE_NOTRACE>".
+    idtac "<PrintAssumptions>".
+    Print Assumptions correct_RAISE_NOTRACE.
+    idtac "</PrintAssumptions>".
+    idtac "</correct_RAISE_NOTRACE>".
+  Abort.
+  Goal True.
+    idtac "<correct_RAISE>".
+    idtac "<PrintAssumptions>".
+    Print Assumptions correct_RAISE.
+    idtac "</PrintAssumptions>".
+    idtac "</correct_RAISE>".
+  Abort.
+  Goal True.
+    idtac "<correct_REPERFORMTERM>".
+    idtac "<PrintAssumptions>".
+    Print Assumptions correct_REPERFORMTERM.
+    idtac "</PrintAssumptions>".
+    idtac "</correct_REPERFORMTERM>".
+  Abort.
+  Goal True.
+    idtac "<correct_RERAISE>".
+    idtac "<PrintAssumptions>".
+    Print Assumptions correct_RERAISE.
+    idtac "</PrintAssumptions>".
+    idtac "</correct_RERAISE>".
+  Abort.
+  Goal True.
+    idtac "<correct_RESTART>".
+    idtac "<PrintAssumptions>".
+    Print Assumptions correct_RESTART.
+    idtac "</PrintAssumptions>".
+    idtac "</correct_RESTART>".
+  Abort.
+  Goal True.
+    idtac "<correct_RESUMETERM>".
+    idtac "<PrintAssumptions>".
+    Print Assumptions correct_RESUMETERM.
+    idtac "</PrintAssumptions>".
+    idtac "</correct_RESUMETERM>".
+  Abort.
+  Goal True.
+    idtac "<correct_RESUME>".
+    idtac "<PrintAssumptions>".
+    Print Assumptions correct_RESUME.
+    idtac "</PrintAssumptions>".
+    idtac "</correct_RESUME>".
+  Abort.
+  Goal True.
+    idtac "<correct_RETURN>".
+    idtac "<PrintAssumptions>".
+    Print Assumptions correct_RETURN.
+    idtac "</PrintAssumptions>".
+    idtac "</correct_RETURN>".
+  Abort.
+  Goal True.
+    idtac "<correct_SETBYTESCHAR>".
+    idtac "<PrintAssumptions>".
+    Print Assumptions correct_SETBYTESCHAR.
+    idtac "</PrintAssumptions>".
+    idtac "</correct_SETBYTESCHAR>".
+  Abort.
+  Goal True.
+    idtac "<correct_SETFIELD0>".
+    idtac "<PrintAssumptions>".
+    Print Assumptions correct_SETFIELD0.
+    idtac "</PrintAssumptions>".
+    idtac "</correct_SETFIELD0>".
+  Abort.
+  Goal True.
+    idtac "<correct_SETFIELD1>".
+    idtac "<PrintAssumptions>".
+    Print Assumptions correct_SETFIELD1.
+    idtac "</PrintAssumptions>".
+    idtac "</correct_SETFIELD1>".
+  Abort.
+  Goal True.
+    idtac "<correct_SETFIELD2>".
+    idtac "<PrintAssumptions>".
+    Print Assumptions correct_SETFIELD2.
+    idtac "</PrintAssumptions>".
+    idtac "</correct_SETFIELD2>".
+  Abort.
+  Goal True.
+    idtac "<correct_SETFIELD3>".
+    idtac "<PrintAssumptions>".
+    Print Assumptions correct_SETFIELD3.
+    idtac "</PrintAssumptions>".
+    idtac "</correct_SETFIELD3>".
+  Abort.
+  Goal True.
+    idtac "<correct_SETFIELD>".
+    idtac "<PrintAssumptions>".
+    Print Assumptions correct_SETFIELD.
+    idtac "</PrintAssumptions>".
+    idtac "</correct_SETFIELD>".
+  Abort.
+  Goal True.
+    idtac "<correct_SETFLOATFIELD>".
+    idtac "<PrintAssumptions>".
+    Print Assumptions correct_SETFLOATFIELD.
+    idtac "</PrintAssumptions>".
+    idtac "</correct_SETFLOATFIELD>".
+  Abort.
+  Goal True.
+    idtac "<correct_SETGLOBAL>".
+    idtac "<PrintAssumptions>".
+    Print Assumptions correct_SETGLOBAL.
+    idtac "</PrintAssumptions>".
+    idtac "</correct_SETGLOBAL>".
+  Abort.
+  Goal True.
+    idtac "<correct_SETVECTITEM>".
+    idtac "<PrintAssumptions>".
+    Print Assumptions correct_SETVECTITEM.
+    idtac "</PrintAssumptions>".
+    idtac "</correct_SETVECTITEM>".
+  Abort.
+  Goal True.
+    idtac "<correct_STOP>".
+    idtac "<PrintAssumptions>".
+    Print Assumptions correct_STOP.
+    idtac "</PrintAssumptions>".
+    idtac "</correct_STOP>".
+  Abort.
+  Goal True.
+    idtac "<correct_SUBINT>".
+    idtac "<PrintAssumptions>".
+    Print Assumptions correct_SUBINT.
+    idtac "</PrintAssumptions>".
+    idtac "</correct_SUBINT>".
+  Abort.
+  Goal True.
+    idtac "<correct_SWITCH>".
+    idtac "<PrintAssumptions>".
+    Print Assumptions correct_SWITCH.
+    idtac "</PrintAssumptions>".
+    idtac "</correct_SWITCH>".
+  Abort.
+  Goal True.
+    idtac "<correct_UGEINT>".
+    idtac "<PrintAssumptions>".
+    Print Assumptions correct_UGEINT.
+    idtac "</PrintAssumptions>".
+    idtac "</correct_UGEINT>".
+  Abort.
+  Goal True.
+    idtac "<correct_ULTINT>".
+    idtac "<PrintAssumptions>".
+    Print Assumptions correct_ULTINT.
+    idtac "</PrintAssumptions>".
+    idtac "</correct_ULTINT>".
+  Abort.
+  Goal True.
+    idtac "<correct_VECTLENGTH>".
+    idtac "<PrintAssumptions>".
+    Print Assumptions correct_VECTLENGTH.
+    idtac "</PrintAssumptions>".
+    idtac "</correct_VECTLENGTH>".
+  Abort.
+  Goal True.
+    idtac "<correct_XORINT>".
+    idtac "<PrintAssumptions>".
+    Print Assumptions correct_XORINT.
+    idtac "</PrintAssumptions>".
+    idtac "</correct_XORINT>".
+  Abort.
+  End __.
 End InstructVerification.
