verified-ocaml/checker/Compile/CompileChecker.v
@@ -4,12 +4,40 @@
    (from semi-auto/), and the correctness proof (from automatic/). *)
 
 From OCamlInterp.Manual.Compile Require Import CompileSpec.
-From OCamlInterp.SemiAutomatic.Interpret Require Import Interpret.
-From OCamlInterp.Automatic.Compile Require Import Compile.
-From OCamlInterp.Automatic.Compile Require Import CompileProof.
+From OCamlInterp.SemiAutomatic.Interpret Require Interpret.
+From OCamlInterp.Automatic.Compile Require Compile.
+From OCamlInterp.Automatic.Compile Require CompileProof.
 
 Module Check <: CompileSpec.
-  Definition compile_program := compile_program.
-  Definition interpret := interpret.
-  Definition compiler_correctness := compiler_correctness.
+  Definition compile_program := OCamlInterp.Automatic.Compile.Compile.compile_program.
+  Definition interpret := OCamlInterp.SemiAutomatic.Interpret.Interpret.interpret.
+  Definition compiler_correctness := OCamlInterp.Automatic.Compile.CompileProof.compiler_correctness.
+
+  Section __.
+  Set Printing All.
+  Set Printing Fully Qualified.
+  Set Printing Depth 10000000000.
+  Set Printing Width 2000.
+  Goal True.
+    idtac "<compile_program>".
+    idtac "<PrintAssumptions>".
+    Print Assumptions compile_program.
+    idtac "</PrintAssumptions>".
+    idtac "</compile_program>".
+  Abort.
+  Goal True.
+    idtac "<interpret>".
+    idtac "<PrintAssumptions>".
+    Print Assumptions interpret.
+    idtac "</PrintAssumptions>".
+    idtac "</interpret>".
+  Abort.
+  Goal True.
+    idtac "<compiler_correctness>".
+    idtac "<PrintAssumptions>".
+    Print Assumptions compiler_correctness.
+    idtac "</PrintAssumptions>".
+    idtac "</compiler_correctness>".
+  Abort.
+  End __.
 End Check.
