verified-ocaml/checker/LexParse/LexParseChecker.v
@@ -3,12 +3,40 @@
    (from semi-auto/) and lex_parse (from automatic/). *)
 
 From OCamlInterp.Manual.LexParse Require Import LexParseSpec.
-From OCamlInterp.Automatic.LexParse Require Import LexParse.
-From OCamlInterp.Automatic.LexParse Require Import LexParseProof.
-From OCamlInterp.SemiAutomatic.LexParse Require Import PrettyPrint.
+From OCamlInterp.Automatic.LexParse Require LexParse.
+From OCamlInterp.Automatic.LexParse Require LexParseProof.
+From OCamlInterp.SemiAutomatic.LexParse Require PrettyPrint.
 
 Module Check <: LexParseSpec.
-  Definition pp_program := pp_program.
-  Definition lex_parse := lex_parse.
-  Definition lex_parse_pp_inverse := lex_parse_pp_inverse.
+  Definition pp_program := OCamlInterp.SemiAutomatic.LexParse.PrettyPrint.pp_program.
+  Definition lex_parse := OCamlInterp.Automatic.LexParse.LexParse.lex_parse.
+  Definition lex_parse_pp_inverse := OCamlInterp.Automatic.LexParse.LexParseProof.lex_parse_pp_inverse.
+
+  Section __.
+  Set Printing All.
+  Set Printing Fully Qualified.
+  Set Printing Depth 10000000000.
+  Set Printing Width 2000.
+  Goal True.
+    idtac "<pp_program>".
+    idtac "<PrintAssumptions>".
+    Print Assumptions pp_program.
+    idtac "</PrintAssumptions>".
+    idtac "</pp_program>".
+  Abort.
+  Goal True.
+    idtac "<lex_parse>".
+    idtac "<PrintAssumptions>".
+    Print Assumptions lex_parse.
+    idtac "</PrintAssumptions>".
+    idtac "</lex_parse>".
+  Abort.
+  Goal True.
+    idtac "<lex_parse_pp_inverse>".
+    idtac "<PrintAssumptions>".
+    Print Assumptions lex_parse_pp_inverse.
+    idtac "</PrintAssumptions>".
+    idtac "</lex_parse_pp_inverse>".
+  Abort.
+  End __.
 End Check.
